PROP_MERGE2 DONE!

fqueue2.fst
@@ -999,14 +999,14 @@ val merge : ltr:ae
                                           (memq e b /\ memq e1 b /\ fst e <> fst e1 /\ order e e1 (tolist b) /\ memq e res /\ memq e1 res) \/
                                           (memq e l /\ mem e1 (diff_s (tolist a) (tolist l)) /\ fst e <> fst e1 /\ memq e res /\ memq e1 res) \/
                                           (memq e l /\ mem e1 (diff_s (tolist b) (tolist l)) /\ fst e <> fst e1 /\ memq e res /\ memq e1 res) \/
-                                          (mem e (diff_s (tolist a) (tolist l)) /\ mem e1 (diff_s (tolist b) (tolist l)) /\ (fst e < fst e1))) <==>
+                                          (((mem e (diff_s (tolist a) (tolist l)) /\ mem e1 (diff_s (tolist b) (tolist l))) \/
+                                            (mem e (diff_s (tolist b) (tolist l)) /\ mem e1 (diff_s (tolist a) (tolist l)))) /\ (fst e < fst e1))) <==>
                                           (memq e res /\ memq e1 res /\ fst e <> fst e1 /\ order e e1 (tolist res)))
                             ))
 
 #push-options "--initial_fuel 6 --ifuel 6 --initial_ifuel 6 --fuel 6 --z3rlimit 10000"
 
 let merge ltr l atr a btr b = admit(); (S (merge_s (tolist l) (tolist a) (tolist b)) [])
-
 
 
 val absmerge01 : ltr:ae
@@ -1056,6 +1056,8 @@ val prop_merge02  : ltr: ae
                               (forall e. mem e atr.l ==> not (member (get_id e) btr.l)) /\
                               (forall e e1. (memq e a /\ memq e1 l /\ (fst e = fst e1)) ==> (snd e = snd e1)) /\
                               (forall e e1. (memq e b /\ memq e1 l /\ (fst e = fst e1)) ==> (snd e = snd e1)) /\
+                              (forall e e1. memq e l /\ mem e1 (diff_s (tolist a) (tolist l)) ==> fst e < fst e1) /\
+                              (forall e e1. memq e l /\ mem e1 (diff_s (tolist b) (tolist l)) ==> fst e < fst e1) /\
                             (forall e e1. mem e (tolist l) /\ mem e1 (tolist l) /\ mem e (tolist a) /\ mem e1 (tolist a) /\ order e e1 (tolist l) ==> order e e1 (tolist a)) /\
                             (forall e e1. mem e (tolist l) /\ mem e1 (tolist l) /\ mem e (tolist b) /\ mem e1 (tolist b) /\ order e e1 (tolist l) ==> order e e1 (tolist b)) /\
                               (forall e e1. (mem e ltr.l /\ mem e1 atr.l ==> get_id e < get_id e1)) /\
@@ -1104,6 +1106,8 @@ val prop_merge01 : ltr: ae
                               (forall e. mem e atr.l ==> not (member (get_id e) btr.l)) /\
                               (forall e e1. (memq e a /\ memq e1 l /\ (fst e = fst e1)) ==> (snd e = snd e1)) /\
                               (forall e e1. (memq e b /\ memq e1 l /\ (fst e = fst e1)) ==> (snd e = snd e1)) /\
+                              (forall e e1. memq e l /\ mem e1 (diff_s (tolist a) (tolist l)) ==> fst e < fst e1) /\
+                              (forall e e1. memq e l /\ mem e1 (diff_s (tolist b) (tolist l)) ==> fst e < fst e1) /\
                             (forall e e1. mem e (tolist l) /\ mem e1 (tolist l) /\ mem e (tolist a) /\ mem e1 (tolist a) /\ order e e1 (tolist l) ==> order e e1 (tolist a)) /\
                             (forall e e1. mem e (tolist l) /\ mem e1 (tolist l) /\ mem e (tolist b) /\ mem e1 (tolist b) /\ order e e1 (tolist l) ==> order e e1 (tolist b)) /\
                               (forall e e1. (mem e ltr.l /\ mem e1 atr.l ==> get_id e < get_id e1)) /\
@@ -1155,6 +1159,8 @@ val prop_merge001 : ltr: ae
                               (forall e. mem e atr.l ==> not (member (get_id e) btr.l)) /\
                               (forall e e1. (memq e a /\ memq e1 l /\ (fst e = fst e1)) ==> (snd e = snd e1)) /\
                               (forall e e1. (memq e b /\ memq e1 l /\ (fst e = fst e1)) ==> (snd e = snd e1)) /\
+                              (forall e e1. memq e l /\ mem e1 (diff_s (tolist a) (tolist l)) ==> fst e < fst e1) /\
+                              (forall e e1. memq e l /\ mem e1 (diff_s (tolist b) (tolist l)) ==> fst e < fst e1) /\
                             (forall e e1. mem e (tolist l) /\ mem e1 (tolist l) /\ mem e (tolist a) /\ mem e1 (tolist a) /\ order e e1 (tolist l) ==> order e e1 (tolist a)) /\
                             (forall e e1. mem e (tolist l) /\ mem e1 (tolist l) /\ mem e (tolist b) /\ mem e1 (tolist b) /\ order e e1 (tolist l) ==> order e e1 (tolist b)) /\
                               (forall e e1. (mem e ltr.l /\ mem e1 atr.l ==> get_id e < get_id e1)) /\
@@ -1199,6 +1205,8 @@ val prop_merge002 : ltr: ae
                               (forall e. mem e atr.l ==> not (member (get_id e) btr.l)) /\
                               (forall e e1. (memq e a /\ memq e1 l /\ (fst e = fst e1)) ==> (snd e = snd e1)) /\
                               (forall e e1. (memq e b /\ memq e1 l /\ (fst e = fst e1)) ==> (snd e = snd e1)) /\
+                              (forall e e1. memq e l /\ mem e1 (diff_s (tolist a) (tolist l)) ==> fst e < fst e1) /\
+                              (forall e e1. memq e l /\ mem e1 (diff_s (tolist b) (tolist l)) ==> fst e < fst e1) /\
                             (forall e e1. mem e (tolist l) /\ mem e1 (tolist l) /\ mem e (tolist a) /\ mem e1 (tolist a) /\ order e e1 (tolist l) ==> order e e1 (tolist a)) /\
                             (forall e e1. mem e (tolist l) /\ mem e1 (tolist l) /\ mem e (tolist b) /\ mem e1 (tolist b) /\ order e e1 (tolist l) ==> order e e1 (tolist b)) /\
                               (forall e e1. (mem e ltr.l /\ mem e1 atr.l ==> get_id e < get_id e1)) /\
@@ -1251,6 +1259,8 @@ val prop_merge0 : ltr: ae
                               (forall e. mem e atr.l ==> not (member (get_id e) btr.l)) /\
                               (forall e e1. (memq e a /\ memq e1 l /\ (fst e = fst e1)) ==> (snd e = snd e1)) /\
                               (forall e e1. (memq e b /\ memq e1 l /\ (fst e = fst e1)) ==> (snd e = snd e1)) /\
+                              (forall e e1. memq e l /\ mem e1 (diff_s (tolist a) (tolist l)) ==> fst e < fst e1) /\
+                              (forall e e1. memq e l /\ mem e1 (diff_s (tolist b) (tolist l)) ==> fst e < fst e1) /\
                             (forall e e1. mem e (tolist l) /\ mem e1 (tolist l) /\ mem e (tolist a) /\ mem e1 (tolist a) /\ order e e1 (tolist l) ==> order e e1 (tolist a)) /\
                             (forall e e1. mem e (tolist l) /\ mem e1 (tolist l) /\ mem e (tolist b) /\ mem e1 (tolist b) /\ order e e1 (tolist l) ==> order e e1 (tolist b)) /\
                               (forall e e1. (mem e ltr.l /\ mem e1 atr.l ==> get_id e < get_id e1)) /\
@@ -1276,7 +1286,7 @@ let prop_merge0 ltr l atr a btr b =
                     forall_mem enq_list (fun x -> mem x tr.l && is_enqueue x && mem ((get_id x), (get_ele x)) (tolist s0)));
   ()
 
-val prop_merge1 : ltr: ae
+val prop_merge21 : ltr: ae
                 -> l:s
                 -> atr:ae
                 -> a:s
@@ -1287,39 +1297,484 @@ val prop_merge1 : ltr: ae
                               (forall e. mem e atr.l ==> not (member (get_id e) btr.l)) /\
                               (forall e e1. (memq e a /\ memq e1 l /\ (fst e = fst e1)) ==> (snd e = snd e1)) /\
                               (forall e e1. (memq e b /\ memq e1 l /\ (fst e = fst e1)) ==> (snd e = snd e1)) /\
+                              (forall e e1. memq e l /\ mem e1 (diff_s (tolist a) (tolist l)) ==> fst e < fst e1) /\
+                              (forall e e1. memq e l /\ mem e1 (diff_s (tolist b) (tolist l)) ==> fst e < fst e1) /\
                             (forall e e1. mem e (tolist l) /\ mem e1 (tolist l) /\ mem e (tolist a) /\ mem e1 (tolist a) /\ order e e1 (tolist l) ==> order e e1 (tolist a)) /\
                             (forall e e1. mem e (tolist l) /\ mem e1 (tolist l) /\ mem e (tolist b) /\ mem e1 (tolist b) /\ order e e1 (tolist l) ==> order e e1 (tolist b)) /\
                               (forall e e1. (mem e ltr.l /\ mem e1 atr.l ==> get_id e < get_id e1)) /\
                               (forall e e1. (mem e ltr.l /\ mem e1 btr.l ==> get_id e < get_id e1)) /\
                               (sim ltr l /\ sim (union ltr atr) a /\ sim (union ltr btr) b) /\
-                              (forall e. mem_id e (diff_s (tolist a) (tolist l)) ==> not (mem_id e (diff_s (tolist b) (tolist l))))/\
-                              (forall e. mem_id e (diff_s (tolist b) (tolist l)) ==> not (mem_id e (diff_s (tolist a) (tolist l))))))
-                       (ensures (sim1 (absmerge ltr atr btr) (merge ltr l atr a btr b)))
+                              (forall e. mem_id e (diff_s (tolist a) (tolist l)) ==> not (mem_id e (diff_s (tolist b) (tolist l)))) /\
+                              (forall e. mem_id e (diff_s (tolist b) (tolist l)) ==> not (mem_id e (diff_s (tolist a) (tolist l))))) /\
+                              (sim0 (absmerge ltr atr btr) (merge ltr l atr a btr b)))
+                       (ensures (forall e e1. mem e (filter_op (fun x -> is_enqueue x && mem x atr.l && not
+                             (exists_mem atr.l (fun d -> is_dequeue d && mem d atr.l && mem x atr.l && get_id x <> get_id d && matched x d atr))) atr.l) /\
+                               mem e1 (filter_op (fun x -> is_enqueue x && mem x atr.l && not
+                             (exists_mem atr.l (fun d -> is_dequeue d && mem d atr.l && mem x atr.l && get_id x <> get_id d && matched x d atr))) atr.l) /\
+                               get_id e <> get_id e1 /\ mem e1
+                             (filter_op (fun e1 -> get_id e <> get_id e1 && ((absmerge ltr atr btr).vis e e1)) (filter_op (fun x ->
+                               is_enqueue x && mem x (absmerge ltr atr btr).l && not
+                             (exists_mem (absmerge ltr atr btr).l (fun d -> is_dequeue d && mem d (absmerge ltr atr btr).l && mem x (absmerge ltr atr btr).l &&
+                               get_id x <> get_id d && matched x d (absmerge ltr atr btr)))) (absmerge ltr atr btr).l)) ==>
+                          (memq ((get_id e), (get_ele e)) (merge ltr l atr a btr b) /\ memq ((get_id e1), (get_ele e1)) (merge ltr l atr a btr b) /\
+                                get_id e <> get_id e1 /\ order ((get_id e), (get_ele e)) ((get_id e1), (get_ele e1)) (tolist (merge ltr l atr a btr b))
+                                      )))
 
-let prop_merge1 ltr l atr a btr b =
+let prop_merge21 ltr l atr a btr b =
   axiom_ae ltr; axiom_ae atr; axiom_ae btr; axiom_ae (union ltr atr); axiom_ae (union ltr btr);
-  prop_merge01 ltr l atr a btr b; prop_merge0 ltr l atr a btr b;
+  prop_merge01 ltr l atr a btr b; prop_merge001 ltr l atr a btr b; prop_merge002 ltr l atr a btr b; prop_merge0 ltr l atr a btr b;
   let tr = absmerge ltr atr btr in
   let s0 = merge ltr l atr a btr b in
   let enq_list = filter_op (fun x -> is_enqueue x && mem x tr.l && not
                              (exists_mem tr.l (fun d -> is_dequeue d && mem d tr.l && mem x tr.l && get_id x <> get_id d && matched x d tr))) tr.l in
 
-  // let enq_list1 = filter_op (fun x -> is_enqueue x && mem x ltr.l && not
-  //                            (exists_mem ltr.l (fun d -> is_dequeue d && mem d ltr.l && mem x ltr.l && get_id x <> get_id d && matched x d ltr))) ltr.l in
+  let enq_list4 = filter_op (fun x -> is_enqueue x && mem x atr.l && not
+                             (exists_mem atr.l (fun d -> is_dequeue d && mem d atr.l && mem x atr.l && get_id x <> get_id d && matched x d atr))) atr.l in
 
-  // let enq_list2 = filter_op (fun x -> is_enqueue x && mem x (union ltr atr).l && not
-  //                            (exists_mem (union ltr atr).l (fun d -> is_dequeue d && mem d (union ltr atr).l && mem x (union ltr atr).l &&
-  //                                        get_id x <> get_id d && matched x d (union ltr atr)))) (union ltr atr).l in
+  assert(forall e e1. mem e (enq_list4) /\ mem e1 (enq_list4) /\ get_id e <> get_id e1 /\ mem e1
+           (filter_op (fun e1 -> get_id e <> get_id e1 && (tr.vis e e1)) (enq_list)) ==>
+                          (memq ((get_id e), (get_ele e)) s0 /\ memq ((get_id e1), (get_ele e1)) s0 /\ get_id e <> get_id e1 /\
+                                      order ((get_id e), (get_ele e)) ((get_id e1), (get_ele e1)) (tolist s0)
+                                      ));
 
-  // let enq_list3 = filter_op (fun x -> is_enqueue x && mem x (union ltr btr).l && not
-  //                            (exists_mem (union ltr btr).l (fun d -> is_dequeue d && mem d (union ltr btr).l && mem x (union ltr btr).l &&
-  //                                        get_id x <> get_id d && matched x d (union ltr btr)))) (union ltr btr).l in
+  ()
 
-  // let enq_list4 = filter_op (fun x -> is_enqueue x && mem x atr.l && not
-  //                            (exists_mem atr.l (fun d -> is_dequeue d && mem d atr.l && mem x atr.l && get_id x <> get_id d && matched x d atr))) atr.l in
+val prop_merge22 : ltr: ae
+                -> l:s
+                -> atr:ae
+                -> a:s
+                -> btr:ae
+                -> b:s
+                -> Lemma (requires (sorted (tolist l) /\ sorted (tolist a) /\ sorted (tolist b) /\ (forall e. mem e ltr.l ==> not (member (get_id e) atr.l)) /\
+                              (forall e. mem e ltr.l ==> not (member (get_id e) btr.l)) /\
+                              (forall e. mem e atr.l ==> not (member (get_id e) btr.l)) /\
+                              (forall e e1. (memq e a /\ memq e1 l /\ (fst e = fst e1)) ==> (snd e = snd e1)) /\
+                              (forall e e1. (memq e b /\ memq e1 l /\ (fst e = fst e1)) ==> (snd e = snd e1)) /\
+                              (forall e e1. memq e l /\ mem e1 (diff_s (tolist a) (tolist l)) ==> fst e < fst e1) /\
+                              (forall e e1. memq e l /\ mem e1 (diff_s (tolist b) (tolist l)) ==> fst e < fst e1) /\
+                            (forall e e1. mem e (tolist l) /\ mem e1 (tolist l) /\ mem e (tolist a) /\ mem e1 (tolist a) /\ order e e1 (tolist l) ==> order e e1 (tolist a)) /\
+                            (forall e e1. mem e (tolist l) /\ mem e1 (tolist l) /\ mem e (tolist b) /\ mem e1 (tolist b) /\ order e e1 (tolist l) ==> order e e1 (tolist b)) /\
+                              (forall e e1. (mem e ltr.l /\ mem e1 atr.l ==> get_id e < get_id e1)) /\
+                              (forall e e1. (mem e ltr.l /\ mem e1 btr.l ==> get_id e < get_id e1)) /\
+                              (sim ltr l /\ sim (union ltr atr) a /\ sim (union ltr btr) b) /\
+                              (forall e. mem_id e (diff_s (tolist a) (tolist l)) ==> not (mem_id e (diff_s (tolist b) (tolist l)))) /\
+                              (forall e. mem_id e (diff_s (tolist b) (tolist l)) ==> not (mem_id e (diff_s (tolist a) (tolist l))))) /\
+                              (sim0 (absmerge ltr atr btr) (merge ltr l atr a btr b)))
+                       (ensures (forall e e1. mem e (filter_op (fun x -> is_enqueue x && mem x btr.l && not
+                             (exists_mem btr.l (fun d -> is_dequeue d && mem d btr.l && mem x btr.l && get_id x <> get_id d && matched x d btr))) btr.l) /\
+                               mem e1 (filter_op (fun x -> is_enqueue x && mem x btr.l && not
+                             (exists_mem btr.l (fun d -> is_dequeue d && mem d btr.l && mem x btr.l && get_id x <> get_id d && matched x d btr))) btr.l) /\
+                               get_id e <> get_id e1 /\ mem e1
+                             (filter_op (fun e1 -> get_id e <> get_id e1 && ((absmerge ltr atr btr).vis e e1)) (filter_op (fun x ->
+                               is_enqueue x && mem x (absmerge ltr atr btr).l && not
+                             (exists_mem (absmerge ltr atr btr).l (fun d -> is_dequeue d && mem d (absmerge ltr atr btr).l && mem x (absmerge ltr atr btr).l &&
+                               get_id x <> get_id d && matched x d (absmerge ltr atr btr)))) (absmerge ltr atr btr).l)) ==>
+                          (memq ((get_id e), (get_ele e)) (merge ltr l atr a btr b) /\ memq ((get_id e1), (get_ele e1)) (merge ltr l atr a btr b) /\
+                                get_id e <> get_id e1 /\ order ((get_id e), (get_ele e)) ((get_id e1), (get_ele e1)) (tolist (merge ltr l atr a btr b))
+                                      )))
 
-  // let enq_list5 = filter_op (fun x -> is_enqueue x && mem x btr.l && not
-  //                            (exists_mem btr.l (fun d -> is_dequeue d && mem d btr.l && mem x btr.l && get_id x <> get_id d && matched x d btr))) btr.l in
+let prop_merge22 ltr l atr a btr b =
+  axiom_ae ltr; axiom_ae atr; axiom_ae btr; axiom_ae (union ltr atr); axiom_ae (union ltr btr);
+  prop_merge01 ltr l atr a btr b; prop_merge001 ltr l atr a btr b; prop_merge002 ltr l atr a btr b; prop_merge0 ltr l atr a btr b;
+  let tr = absmerge ltr atr btr in
+  let s0 = merge ltr l atr a btr b in
+  let enq_list = filter_op (fun x -> is_enqueue x && mem x tr.l && not
+                             (exists_mem tr.l (fun d -> is_dequeue d && mem d tr.l && mem x tr.l && get_id x <> get_id d && matched x d tr))) tr.l in
+
+  let enq_list5 = filter_op (fun x -> is_enqueue x && mem x btr.l && not
+                             (exists_mem btr.l (fun d -> is_dequeue d && mem d btr.l && mem x btr.l && get_id x <> get_id d && matched x d btr))) btr.l in
+
+  assert(forall e e1. mem e (enq_list5) /\ mem e1 (enq_list5) /\ get_id e <> get_id e1 /\ mem e1
+           (filter_op (fun e1 -> get_id e <> get_id e1 && ((tr.vis e e1))) (enq_list)) ==>
+                          (memq ((get_id e), (get_ele e)) s0 /\ memq ((get_id e1), (get_ele e1)) s0 /\ get_id e <> get_id e1 /\
+                                      order ((get_id e), (get_ele e)) ((get_id e1), (get_ele e1)) (tolist s0)
+                                      ));
+
+  ()
+
+val prop_merge23 : ltr: ae
+                -> l:s
+                -> atr:ae
+                -> a:s
+                -> btr:ae
+                -> b:s
+                -> Lemma (requires (sorted (tolist l) /\ sorted (tolist a) /\ sorted (tolist b) /\ (forall e. mem e ltr.l ==> not (member (get_id e) atr.l)) /\
+                              (forall e. mem e ltr.l ==> not (member (get_id e) btr.l)) /\
+                              (forall e. mem e atr.l ==> not (member (get_id e) btr.l)) /\
+                              (forall e e1. (memq e a /\ memq e1 l /\ (fst e = fst e1)) ==> (snd e = snd e1)) /\
+                              (forall e e1. (memq e b /\ memq e1 l /\ (fst e = fst e1)) ==> (snd e = snd e1)) /\
+                              (forall e e1. memq e l /\ mem e1 (diff_s (tolist a) (tolist l)) ==> fst e < fst e1) /\
+                              (forall e e1. memq e l /\ mem e1 (diff_s (tolist b) (tolist l)) ==> fst e < fst e1) /\
+                            (forall e e1. mem e (tolist l) /\ mem e1 (tolist l) /\ mem e (tolist a) /\ mem e1 (tolist a) /\ order e e1 (tolist l) ==> order e e1 (tolist a)) /\
+                            (forall e e1. mem e (tolist l) /\ mem e1 (tolist l) /\ mem e (tolist b) /\ mem e1 (tolist b) /\ order e e1 (tolist l) ==> order e e1 (tolist b)) /\
+                              (forall e e1. (mem e ltr.l /\ mem e1 atr.l ==> get_id e < get_id e1)) /\
+                              (forall e e1. (mem e ltr.l /\ mem e1 btr.l ==> get_id e < get_id e1)) /\
+                              (sim ltr l /\ sim (union ltr atr) a /\ sim (union ltr btr) b) /\
+                              (forall e. mem_id e (diff_s (tolist a) (tolist l)) ==> not (mem_id e (diff_s (tolist b) (tolist l)))) /\
+                              (forall e. mem_id e (diff_s (tolist b) (tolist l)) ==> not (mem_id e (diff_s (tolist a) (tolist l))))) /\
+                              (sim0 (absmerge ltr atr btr) (merge ltr l atr a btr b)))
+                       (ensures (forall e e1. mem e (filter_op (fun x -> is_enqueue x && mem x btr.l && not
+                             (exists_mem btr.l (fun d -> is_dequeue d && mem d btr.l && mem x btr.l && get_id x <> get_id d && matched x d btr))) btr.l) /\
+                               mem e1 (filter_op (fun x -> is_enqueue x && mem x btr.l && not
+                             (exists_mem btr.l (fun d -> is_dequeue d && mem d btr.l && mem x btr.l && get_id x <> get_id d && matched x d btr))) btr.l) /\
+                               get_id e <> get_id e1 /\ mem e1
+                             (filter_op (fun e1 -> get_id e <> get_id e1 && ((not ((absmerge ltr atr btr).vis e e1 ||
+                               (absmerge ltr atr btr).vis e1 e) && (get_id e < get_id e1)))) (filter_op (fun x ->
+                               is_enqueue x && mem x (absmerge ltr atr btr).l && not
+                             (exists_mem (absmerge ltr atr btr).l (fun d -> is_dequeue d && mem d (absmerge ltr atr btr).l && mem x (absmerge ltr atr btr).l &&
+                               get_id x <> get_id d && matched x d (absmerge ltr atr btr)))) (absmerge ltr atr btr).l)) ==>
+                          (memq ((get_id e), (get_ele e)) (merge ltr l atr a btr b) /\ memq ((get_id e1), (get_ele e1)) (merge ltr l atr a btr b) /\
+                                get_id e <> get_id e1 /\ order ((get_id e), (get_ele e)) ((get_id e1), (get_ele e1)) (tolist (merge ltr l atr a btr b))
+                                      )))
+
+let prop_merge23 ltr l atr a btr b =
+  axiom_ae ltr; axiom_ae atr; axiom_ae btr; axiom_ae (union ltr atr); axiom_ae (union ltr btr);
+  prop_merge01 ltr l atr a btr b; prop_merge001 ltr l atr a btr b; prop_merge002 ltr l atr a btr b; prop_merge0 ltr l atr a btr b;
+  let tr = absmerge ltr atr btr in
+  let s0 = merge ltr l atr a btr b in
+  let enq_list = filter_op (fun x -> is_enqueue x && mem x tr.l && not
+                             (exists_mem tr.l (fun d -> is_dequeue d && mem d tr.l && mem x tr.l && get_id x <> get_id d && matched x d tr))) tr.l in
+
+  let enq_list5 = filter_op (fun x -> is_enqueue x && mem x btr.l && not
+                             (exists_mem btr.l (fun d -> is_dequeue d && mem d btr.l && mem x btr.l && get_id x <> get_id d && matched x d btr))) btr.l in
+
+  assert(forall e e1. mem e (enq_list5) /\ mem e1 (enq_list5) /\ get_id e <> get_id e1 /\ mem e1
+           (filter_op (fun e1 -> get_id e <> get_id e1 && ((not (tr.vis e e1 || tr.vis e1 e) && (get_id e < get_id e1)))) (enq_list)) ==>
+                          (memq ((get_id e), (get_ele e)) s0 /\ memq ((get_id e1), (get_ele e1)) s0 /\ get_id e <> get_id e1 /\
+                                      order ((get_id e), (get_ele e)) ((get_id e1), (get_ele e1)) (tolist s0)
+                                      ));
+
+  ()
+
+val prop_merge24 : ltr: ae
+                -> l:s
+                -> atr:ae
+                -> a:s
+                -> btr:ae
+                -> b:s
+                -> Lemma (requires (sorted (tolist l) /\ sorted (tolist a) /\ sorted (tolist b) /\ (forall e. mem e ltr.l ==> not (member (get_id e) atr.l)) /\
+                              (forall e. mem e ltr.l ==> not (member (get_id e) btr.l)) /\
+                              (forall e. mem e atr.l ==> not (member (get_id e) btr.l)) /\
+                              (forall e e1. (memq e a /\ memq e1 l /\ (fst e = fst e1)) ==> (snd e = snd e1)) /\
+                              (forall e e1. (memq e b /\ memq e1 l /\ (fst e = fst e1)) ==> (snd e = snd e1)) /\
+                              (forall e e1. memq e l /\ mem e1 (diff_s (tolist a) (tolist l)) ==> fst e < fst e1) /\
+                              (forall e e1. memq e l /\ mem e1 (diff_s (tolist b) (tolist l)) ==> fst e < fst e1) /\
+                            (forall e e1. mem e (tolist l) /\ mem e1 (tolist l) /\ mem e (tolist a) /\ mem e1 (tolist a) /\ order e e1 (tolist l) ==> order e e1 (tolist a)) /\
+                            (forall e e1. mem e (tolist l) /\ mem e1 (tolist l) /\ mem e (tolist b) /\ mem e1 (tolist b) /\ order e e1 (tolist l) ==> order e e1 (tolist b)) /\
+                              (forall e e1. (mem e ltr.l /\ mem e1 atr.l ==> get_id e < get_id e1)) /\
+                              (forall e e1. (mem e ltr.l /\ mem e1 btr.l ==> get_id e < get_id e1)) /\
+                              (sim ltr l /\ sim (union ltr atr) a /\ sim (union ltr btr) b) /\
+                              (forall e. mem_id e (diff_s (tolist a) (tolist l)) ==> not (mem_id e (diff_s (tolist b) (tolist l)))) /\
+                              (forall e. mem_id e (diff_s (tolist b) (tolist l)) ==> not (mem_id e (diff_s (tolist a) (tolist l))))) /\
+                              (sim0 (absmerge ltr atr btr) (merge ltr l atr a btr b)))
+                       (ensures (forall e e1. mem e (filter_op (fun x -> is_enqueue x && mem x atr.l && not
+                             (exists_mem atr.l (fun d -> is_dequeue d && mem d atr.l && mem x atr.l && get_id x <> get_id d && matched x d atr))) atr.l) /\
+                               mem e1 (filter_op (fun x -> is_enqueue x && mem x atr.l && not
+                             (exists_mem atr.l (fun d -> is_dequeue d && mem d atr.l && mem x atr.l && get_id x <> get_id d && matched x d atr))) atr.l) /\
+                               get_id e <> get_id e1 /\ mem e1
+                             (filter_op (fun e1 -> get_id e <> get_id e1 && ((not ((absmerge ltr atr btr).vis e e1 ||
+                               (absmerge ltr atr btr).vis e1 e) && (get_id e < get_id e1)))) (filter_op (fun x ->
+                               is_enqueue x && mem x (absmerge ltr atr btr).l && not
+                             (exists_mem (absmerge ltr atr btr).l (fun d -> is_dequeue d && mem d (absmerge ltr atr btr).l && mem x (absmerge ltr atr btr).l &&
+                               get_id x <> get_id d && matched x d (absmerge ltr atr btr)))) (absmerge ltr atr btr).l)) ==>
+                          (memq ((get_id e), (get_ele e)) (merge ltr l atr a btr b) /\ memq ((get_id e1), (get_ele e1)) (merge ltr l atr a btr b) /\
+                                get_id e <> get_id e1 /\ order ((get_id e), (get_ele e)) ((get_id e1), (get_ele e1)) (tolist (merge ltr l atr a btr b))
+                                      )))
+
+let prop_merge24 ltr l atr a btr b =
+  axiom_ae ltr; axiom_ae atr; axiom_ae btr; axiom_ae (union ltr atr); axiom_ae (union ltr btr);
+  prop_merge01 ltr l atr a btr b; prop_merge001 ltr l atr a btr b; prop_merge002 ltr l atr a btr b; prop_merge0 ltr l atr a btr b;
+  let tr = absmerge ltr atr btr in
+  let s0 = merge ltr l atr a btr b in
+  let enq_list = filter_op (fun x -> is_enqueue x && mem x tr.l && not
+                             (exists_mem tr.l (fun d -> is_dequeue d && mem d tr.l && mem x tr.l && get_id x <> get_id d && matched x d tr))) tr.l in
+
+  let enq_list4 = filter_op (fun x -> is_enqueue x && mem x atr.l && not
+                             (exists_mem atr.l (fun d -> is_dequeue d && mem d atr.l && mem x atr.l && get_id x <> get_id d && matched x d atr))) atr.l in
+
+  assert(forall e e1. mem e (enq_list4) /\ mem e1 (enq_list4) /\ get_id e <> get_id e1 /\ mem e1
+           (filter_op (fun e1 -> get_id e <> get_id e1 && ((not (tr.vis e e1 || tr.vis e1 e) && (get_id e < get_id e1)))) (enq_list)) ==>
+                          (memq ((get_id e), (get_ele e)) s0 /\ memq ((get_id e1), (get_ele e1)) s0 /\ get_id e <> get_id e1 /\
+                                      order ((get_id e), (get_ele e)) ((get_id e1), (get_ele e1)) (tolist s0)
+                                      ));
+
+  ()
+
+
+val prop_merge25 : ltr: ae
+                -> l:s
+                -> atr:ae
+                -> a:s
+                -> btr:ae
+                -> b:s
+                -> Lemma (requires (sorted (tolist l) /\ sorted (tolist a) /\ sorted (tolist b) /\ (forall e. mem e ltr.l ==> not (member (get_id e) atr.l)) /\
+                              (forall e. mem e ltr.l ==> not (member (get_id e) btr.l)) /\
+                              (forall e. mem e atr.l ==> not (member (get_id e) btr.l)) /\
+                              (forall e e1. (memq e a /\ memq e1 l /\ (fst e = fst e1)) ==> (snd e = snd e1)) /\
+                              (forall e e1. (memq e b /\ memq e1 l /\ (fst e = fst e1)) ==> (snd e = snd e1)) /\
+                              (forall e e1. memq e l /\ mem e1 (diff_s (tolist a) (tolist l)) ==> fst e < fst e1) /\
+                              (forall e e1. memq e l /\ mem e1 (diff_s (tolist b) (tolist l)) ==> fst e < fst e1) /\
+                            (forall e e1. mem e (tolist l) /\ mem e1 (tolist l) /\ mem e (tolist a) /\ mem e1 (tolist a) /\ order e e1 (tolist l) ==> order e e1 (tolist a)) /\
+                            (forall e e1. mem e (tolist l) /\ mem e1 (tolist l) /\ mem e (tolist b) /\ mem e1 (tolist b) /\ order e e1 (tolist l) ==> order e e1 (tolist b)) /\
+                              (forall e e1. (mem e ltr.l /\ mem e1 atr.l ==> get_id e < get_id e1)) /\
+                              (forall e e1. (mem e ltr.l /\ mem e1 btr.l ==> get_id e < get_id e1)) /\
+                              (sim ltr l /\ sim (union ltr atr) a /\ sim (union ltr btr) b) /\
+                              (forall e. mem_id e (diff_s (tolist a) (tolist l)) ==> not (mem_id e (diff_s (tolist b) (tolist l)))) /\
+                              (forall e. mem_id e (diff_s (tolist b) (tolist l)) ==> not (mem_id e (diff_s (tolist a) (tolist l))))) /\
+                              (sim0 (absmerge ltr atr btr) (merge ltr l atr a btr b)))
+                       (ensures (forall e e1. mem e (filter_op (fun x -> is_enqueue x && mem x btr.l && not
+                             (exists_mem btr.l (fun d -> is_dequeue d && mem d btr.l && mem x btr.l && get_id x <> get_id d && matched x d btr))) btr.l) /\
+                               mem e1 (filter_op (fun x -> is_enqueue x && mem x atr.l && not
+                             (exists_mem atr.l (fun d -> is_dequeue d && mem d atr.l && mem x atr.l && get_id x <> get_id d && matched x d atr))) atr.l) /\
+                               get_id e <> get_id e1 /\ mem e1
+                             (filter_op (fun e1 -> get_id e <> get_id e1 && ((absmerge ltr atr btr).vis e e1)) (filter_op (fun x ->
+                               is_enqueue x && mem x (absmerge ltr atr btr).l && not
+                             (exists_mem (absmerge ltr atr btr).l (fun d -> is_dequeue d && mem d (absmerge ltr atr btr).l && mem x (absmerge ltr atr btr).l &&
+                               get_id x <> get_id d && matched x d (absmerge ltr atr btr)))) (absmerge ltr atr btr).l)) ==>
+                          (memq ((get_id e), (get_ele e)) (merge ltr l atr a btr b) /\ memq ((get_id e1), (get_ele e1)) (merge ltr l atr a btr b) /\
+                                get_id e <> get_id e1 /\ order ((get_id e), (get_ele e)) ((get_id e1), (get_ele e1)) (tolist (merge ltr l atr a btr b))
+                                      )))
+
+let prop_merge25 ltr l atr a btr b =
+  axiom_ae ltr; axiom_ae atr; axiom_ae btr; axiom_ae (union ltr atr); axiom_ae (union ltr btr);
+  prop_merge01 ltr l atr a btr b; prop_merge001 ltr l atr a btr b; prop_merge002 ltr l atr a btr b; prop_merge0 ltr l atr a btr b;
+  let tr = absmerge ltr atr btr in
+  let s0 = merge ltr l atr a btr b in
+  let enq_list = filter_op (fun x -> is_enqueue x && mem x tr.l && not
+                             (exists_mem tr.l (fun d -> is_dequeue d && mem d tr.l && mem x tr.l && get_id x <> get_id d && matched x d tr))) tr.l in
+
+  let enq_list4 = filter_op (fun x -> is_enqueue x && mem x atr.l && not
+                             (exists_mem atr.l (fun d -> is_dequeue d && mem d atr.l && mem x atr.l && get_id x <> get_id d && matched x d atr))) atr.l in
+
+  let enq_list5 = filter_op (fun x -> is_enqueue x && mem x btr.l && not
+                             (exists_mem btr.l (fun d -> is_dequeue d && mem d btr.l && mem x btr.l && get_id x <> get_id d && matched x d btr))) btr.l in
+
+  assert(forall e e1. mem e (enq_list5) /\ mem e1 (enq_list4) /\ get_id e <> get_id e1 /\ mem e1
+           (filter_op (fun e1 -> get_id e <> get_id e1 && (tr.vis e e1)) (enq_list)) ==>
+                          (memq ((get_id e), (get_ele e)) s0 /\ memq ((get_id e1), (get_ele e1)) s0 /\ get_id e <> get_id e1 /\
+                                      order ((get_id e), (get_ele e)) ((get_id e1), (get_ele e1)) (tolist s0)
+                                      ));
+
+  ()
+
+val prop_merge26 : ltr: ae
+                -> l:s
+                -> atr:ae
+                -> a:s
+                -> btr:ae
+                -> b:s
+                -> Lemma (requires (sorted (tolist l) /\ sorted (tolist a) /\ sorted (tolist b) /\ (forall e. mem e ltr.l ==> not (member (get_id e) atr.l)) /\
+                              (forall e. mem e ltr.l ==> not (member (get_id e) btr.l)) /\
+                              (forall e. mem e atr.l ==> not (member (get_id e) btr.l)) /\
+                              (forall e e1. (memq e a /\ memq e1 l /\ (fst e = fst e1)) ==> (snd e = snd e1)) /\
+                              (forall e e1. (memq e b /\ memq e1 l /\ (fst e = fst e1)) ==> (snd e = snd e1)) /\
+                              (forall e e1. memq e l /\ mem e1 (diff_s (tolist a) (tolist l)) ==> fst e < fst e1) /\
+                              (forall e e1. memq e l /\ mem e1 (diff_s (tolist b) (tolist l)) ==> fst e < fst e1) /\
+                            (forall e e1. mem e (tolist l) /\ mem e1 (tolist l) /\ mem e (tolist a) /\ mem e1 (tolist a) /\ order e e1 (tolist l) ==> order e e1 (tolist a)) /\
+                            (forall e e1. mem e (tolist l) /\ mem e1 (tolist l) /\ mem e (tolist b) /\ mem e1 (tolist b) /\ order e e1 (tolist l) ==> order e e1 (tolist b)) /\
+                              (forall e e1. (mem e ltr.l /\ mem e1 atr.l ==> get_id e < get_id e1)) /\
+                              (forall e e1. (mem e ltr.l /\ mem e1 btr.l ==> get_id e < get_id e1)) /\
+                              (sim ltr l /\ sim (union ltr atr) a /\ sim (union ltr btr) b) /\
+                              (forall e. mem_id e (diff_s (tolist a) (tolist l)) ==> not (mem_id e (diff_s (tolist b) (tolist l)))) /\
+                              (forall e. mem_id e (diff_s (tolist b) (tolist l)) ==> not (mem_id e (diff_s (tolist a) (tolist l))))) /\
+                              (sim0 (absmerge ltr atr btr) (merge ltr l atr a btr b)))
+                       (ensures (forall e e1. mem e (filter_op (fun x -> is_enqueue x && mem x atr.l && not
+                             (exists_mem atr.l (fun d -> is_dequeue d && mem d atr.l && mem x atr.l && get_id x <> get_id d && matched x d atr))) atr.l) /\
+                               mem e1 (filter_op (fun x -> is_enqueue x && mem x btr.l && not
+                             (exists_mem btr.l (fun d -> is_dequeue d && mem d btr.l && mem x btr.l && get_id x <> get_id d && matched x d btr))) btr.l) /\
+                               get_id e <> get_id e1 /\ mem e1
+                             (filter_op (fun e1 -> get_id e <> get_id e1 && ((absmerge ltr atr btr).vis e e1)) (filter_op (fun x ->
+                               is_enqueue x && mem x (absmerge ltr atr btr).l && not
+                             (exists_mem (absmerge ltr atr btr).l (fun d -> is_dequeue d && mem d (absmerge ltr atr btr).l && mem x (absmerge ltr atr btr).l &&
+                               get_id x <> get_id d && matched x d (absmerge ltr atr btr)))) (absmerge ltr atr btr).l)) ==>
+                          (memq ((get_id e), (get_ele e)) (merge ltr l atr a btr b) /\ memq ((get_id e1), (get_ele e1)) (merge ltr l atr a btr b) /\
+                                get_id e <> get_id e1 /\ order ((get_id e), (get_ele e)) ((get_id e1), (get_ele e1)) (tolist (merge ltr l atr a btr b))
+                                      )))
+
+let prop_merge26 ltr l atr a btr b =
+  axiom_ae ltr; axiom_ae atr; axiom_ae btr; axiom_ae (union ltr atr); axiom_ae (union ltr btr);
+  prop_merge01 ltr l atr a btr b; prop_merge001 ltr l atr a btr b; prop_merge002 ltr l atr a btr b; prop_merge0 ltr l atr a btr b;
+  let tr = absmerge ltr atr btr in
+  let s0 = merge ltr l atr a btr b in
+  let enq_list = filter_op (fun x -> is_enqueue x && mem x tr.l && not
+                             (exists_mem tr.l (fun d -> is_dequeue d && mem d tr.l && mem x tr.l && get_id x <> get_id d && matched x d tr))) tr.l in
+
+  let enq_list4 = filter_op (fun x -> is_enqueue x && mem x atr.l && not
+                             (exists_mem atr.l (fun d -> is_dequeue d && mem d atr.l && mem x atr.l && get_id x <> get_id d && matched x d atr))) atr.l in
+
+  let enq_list5 = filter_op (fun x -> is_enqueue x && mem x btr.l && not
+                             (exists_mem btr.l (fun d -> is_dequeue d && mem d btr.l && mem x btr.l && get_id x <> get_id d && matched x d btr))) btr.l in
+
+  assert(forall e e1. mem e (enq_list4) /\ mem e1 (enq_list5) /\ get_id e <> get_id e1 /\ mem e1
+           (filter_op (fun e1 -> get_id e <> get_id e1 && ((tr.vis e e1))) (enq_list)) ==>
+                          (memq ((get_id e), (get_ele e)) s0 /\ memq ((get_id e1), (get_ele e1)) s0 /\ get_id e <> get_id e1 /\
+                                      order ((get_id e), (get_ele e)) ((get_id e1), (get_ele e1)) (tolist s0)
+                                      ));
+
+  ()
+
+val prop_merge27 : ltr: ae
+                -> l:s
+                -> atr:ae
+                -> a:s
+                -> btr:ae
+                -> b:s
+                -> Lemma (requires (sorted (tolist l) /\ sorted (tolist a) /\ sorted (tolist b) /\ (forall e. mem e ltr.l ==> not (member (get_id e) atr.l)) /\
+                              (forall e. mem e ltr.l ==> not (member (get_id e) btr.l)) /\
+                              (forall e. mem e atr.l ==> not (member (get_id e) btr.l)) /\
+                              (forall e e1. (memq e a /\ memq e1 l /\ (fst e = fst e1)) ==> (snd e = snd e1)) /\
+                              (forall e e1. (memq e b /\ memq e1 l /\ (fst e = fst e1)) ==> (snd e = snd e1)) /\
+                              (forall e e1. memq e l /\ mem e1 (diff_s (tolist a) (tolist l)) ==> fst e < fst e1) /\
+                              (forall e e1. memq e l /\ mem e1 (diff_s (tolist b) (tolist l)) ==> fst e < fst e1) /\
+                            (forall e e1. mem e (tolist l) /\ mem e1 (tolist l) /\ mem e (tolist a) /\ mem e1 (tolist a) /\ order e e1 (tolist l) ==> order e e1 (tolist a)) /\
+                            (forall e e1. mem e (tolist l) /\ mem e1 (tolist l) /\ mem e (tolist b) /\ mem e1 (tolist b) /\ order e e1 (tolist l) ==> order e e1 (tolist b)) /\
+                              (forall e e1. (mem e ltr.l /\ mem e1 atr.l ==> get_id e < get_id e1)) /\
+                              (forall e e1. (mem e ltr.l /\ mem e1 btr.l ==> get_id e < get_id e1)) /\
+                              (sim ltr l /\ sim (union ltr atr) a /\ sim (union ltr btr) b) /\
+                              (forall e. mem_id e (diff_s (tolist a) (tolist l)) ==> not (mem_id e (diff_s (tolist b) (tolist l)))) /\
+                              (forall e. mem_id e (diff_s (tolist b) (tolist l)) ==> not (mem_id e (diff_s (tolist a) (tolist l))))) /\
+                              (sim0 (absmerge ltr atr btr) (merge ltr l atr a btr b)))
+                       (ensures (forall e e1. mem e (filter_op (fun x -> is_enqueue x && mem x atr.l && not
+                             (exists_mem atr.l (fun d -> is_dequeue d && mem d atr.l && mem x atr.l && get_id x <> get_id d && matched x d atr))) atr.l) /\
+                               mem e1 (filter_op (fun x -> is_enqueue x && mem x btr.l && not
+                             (exists_mem btr.l (fun d -> is_dequeue d && mem d btr.l && mem x btr.l && get_id x <> get_id d && matched x d btr))) btr.l) /\
+                               get_id e <> get_id e1 /\ mem e1
+                             (filter_op (fun e1 -> get_id e <> get_id e1 && ((not ((absmerge ltr atr btr).vis e e1 ||
+                               (absmerge ltr atr btr).vis e1 e) && (get_id e < get_id e1)))) (filter_op (fun x ->
+                               is_enqueue x && mem x (absmerge ltr atr btr).l && not
+                             (exists_mem (absmerge ltr atr btr).l (fun d -> is_dequeue d && mem d (absmerge ltr atr btr).l && mem x (absmerge ltr atr btr).l &&
+                               get_id x <> get_id d && matched x d (absmerge ltr atr btr)))) (absmerge ltr atr btr).l)) ==>
+                          (memq ((get_id e), (get_ele e)) (merge ltr l atr a btr b) /\ memq ((get_id e1), (get_ele e1)) (merge ltr l atr a btr b) /\
+                                get_id e <> get_id e1 /\ order ((get_id e), (get_ele e)) ((get_id e1), (get_ele e1)) (tolist (merge ltr l atr a btr b))
+                                      )))
+
+let prop_merge27 ltr l atr a btr b =
+  axiom_ae ltr; axiom_ae atr; axiom_ae btr; axiom_ae (union ltr atr); axiom_ae (union ltr btr);
+  prop_merge01 ltr l atr a btr b; prop_merge001 ltr l atr a btr b; prop_merge002 ltr l atr a btr b; prop_merge0 ltr l atr a btr b;
+  let tr = absmerge ltr atr btr in
+  let s0 = merge ltr l atr a btr b in
+  let enq_list = filter_op (fun x -> is_enqueue x && mem x tr.l && not
+                             (exists_mem tr.l (fun d -> is_dequeue d && mem d tr.l && mem x tr.l && get_id x <> get_id d && matched x d tr))) tr.l in
+
+  let enq_list4 = filter_op (fun x -> is_enqueue x && mem x atr.l && not
+                             (exists_mem atr.l (fun d -> is_dequeue d && mem d atr.l && mem x atr.l && get_id x <> get_id d && matched x d atr))) atr.l in
+
+  let enq_list5 = filter_op (fun x -> is_enqueue x && mem x btr.l && not
+                             (exists_mem btr.l (fun d -> is_dequeue d && mem d btr.l && mem x btr.l && get_id x <> get_id d && matched x d btr))) btr.l in
+
+  assert(forall e e1. mem e (enq_list4) /\ mem e1 (enq_list5) /\ get_id e <> get_id e1 /\ mem e1
+           (filter_op (fun e1 -> get_id e <> get_id e1 && ((not (tr.vis e e1 || tr.vis e1 e) && (get_id e < get_id e1)))) (enq_list)) ==>
+                          (memq ((get_id e), (get_ele e)) s0 /\ memq ((get_id e1), (get_ele e1)) s0 /\ get_id e <> get_id e1 /\
+                                      order ((get_id e), (get_ele e)) ((get_id e1), (get_ele e1)) (tolist s0)
+                                      ));
+
+  ()
+
+val prop_merge28 : ltr: ae
+                -> l:s
+                -> atr:ae
+                -> a:s
+                -> btr:ae
+                -> b:s
+                -> Lemma (requires (sorted (tolist l) /\ sorted (tolist a) /\ sorted (tolist b) /\ (forall e. mem e ltr.l ==> not (member (get_id e) atr.l)) /\
+                              (forall e. mem e ltr.l ==> not (member (get_id e) btr.l)) /\
+                              (forall e. mem e atr.l ==> not (member (get_id e) btr.l)) /\
+                              (forall e e1. (memq e a /\ memq e1 l /\ (fst e = fst e1)) ==> (snd e = snd e1)) /\
+                              (forall e e1. (memq e b /\ memq e1 l /\ (fst e = fst e1)) ==> (snd e = snd e1)) /\
+                              (forall e e1. memq e l /\ mem e1 (diff_s (tolist a) (tolist l)) ==> fst e < fst e1) /\
+                              (forall e e1. memq e l /\ mem e1 (diff_s (tolist b) (tolist l)) ==> fst e < fst e1) /\
+                            (forall e e1. mem e (tolist l) /\ mem e1 (tolist l) /\ mem e (tolist a) /\ mem e1 (tolist a) /\ order e e1 (tolist l) ==> order e e1 (tolist a)) /\
+                            (forall e e1. mem e (tolist l) /\ mem e1 (tolist l) /\ mem e (tolist b) /\ mem e1 (tolist b) /\ order e e1 (tolist l) ==> order e e1 (tolist b)) /\
+                              (forall e e1. (mem e ltr.l /\ mem e1 atr.l ==> get_id e < get_id e1)) /\
+                              (forall e e1. (mem e ltr.l /\ mem e1 btr.l ==> get_id e < get_id e1)) /\
+                              (sim ltr l /\ sim (union ltr atr) a /\ sim (union ltr btr) b) /\
+                              (forall e. mem_id e (diff_s (tolist a) (tolist l)) ==> not (mem_id e (diff_s (tolist b) (tolist l)))) /\
+                              (forall e. mem_id e (diff_s (tolist b) (tolist l)) ==> not (mem_id e (diff_s (tolist a) (tolist l))))) /\
+                              (sim0 (absmerge ltr atr btr) (merge ltr l atr a btr b)))
+                       (ensures (forall e e1. mem e (filter_op (fun x -> is_enqueue x && mem x btr.l && not
+                             (exists_mem btr.l (fun d -> is_dequeue d && mem d btr.l && mem x btr.l && get_id x <> get_id d && matched x d btr))) btr.l) /\
+                               mem e1 (filter_op (fun x -> is_enqueue x && mem x atr.l && not
+                             (exists_mem atr.l (fun d -> is_dequeue d && mem d atr.l && mem x atr.l && get_id x <> get_id d && matched x d atr))) atr.l) /\
+                               get_id e <> get_id e1 /\ mem e1
+                             (filter_op (fun e1 -> get_id e <> get_id e1 && ((not ((absmerge ltr atr btr).vis e e1 ||
+                               (absmerge ltr atr btr).vis e1 e) && (get_id e < get_id e1)))) (filter_op (fun x ->
+                               is_enqueue x && mem x (absmerge ltr atr btr).l && not
+                             (exists_mem (absmerge ltr atr btr).l (fun d -> is_dequeue d && mem d (absmerge ltr atr btr).l && mem x (absmerge ltr atr btr).l &&
+                               get_id x <> get_id d && matched x d (absmerge ltr atr btr)))) (absmerge ltr atr btr).l)) ==>
+                          (memq ((get_id e), (get_ele e)) (merge ltr l atr a btr b) /\ memq ((get_id e1), (get_ele e1)) (merge ltr l atr a btr b) /\
+                                get_id e <> get_id e1 /\ order ((get_id e), (get_ele e)) ((get_id e1), (get_ele e1)) (tolist (merge ltr l atr a btr b))
+                                      )))
+
+let prop_merge28 ltr l atr a btr b =
+  axiom_ae ltr; axiom_ae atr; axiom_ae btr; axiom_ae (union ltr atr); axiom_ae (union ltr btr);
+  prop_merge01 ltr l atr a btr b; prop_merge001 ltr l atr a btr b; prop_merge002 ltr l atr a btr b; prop_merge0 ltr l atr a btr b;
+  let tr = absmerge ltr atr btr in
+  let s0 = merge ltr l atr a btr b in
+  let enq_list = filter_op (fun x -> is_enqueue x && mem x tr.l && not
+                             (exists_mem tr.l (fun d -> is_dequeue d && mem d tr.l && mem x tr.l && get_id x <> get_id d && matched x d tr))) tr.l in
+
+  let enq_list4 = filter_op (fun x -> is_enqueue x && mem x atr.l && not
+                             (exists_mem atr.l (fun d -> is_dequeue d && mem d atr.l && mem x atr.l && get_id x <> get_id d && matched x d atr))) atr.l in
+
+  let enq_list5 = filter_op (fun x -> is_enqueue x && mem x btr.l && not
+                             (exists_mem btr.l (fun d -> is_dequeue d && mem d btr.l && mem x btr.l && get_id x <> get_id d && matched x d btr))) btr.l in
+
+  assert(forall e e1. mem e (enq_list5) /\ mem e1 (enq_list4) /\ get_id e <> get_id e1 /\ mem e1
+           (filter_op (fun e1 -> get_id e <> get_id e1 && ((not (tr.vis e e1 || tr.vis e1 e) && (get_id e < get_id e1)))) (enq_list)) ==>
+                          (memq ((get_id e), (get_ele e)) s0 /\ memq ((get_id e1), (get_ele e1)) s0 /\ get_id e <> get_id e1 /\
+                                      order ((get_id e), (get_ele e)) ((get_id e1), (get_ele e1)) (tolist s0)
+                                      ));
+
+  ()
+
+val prop_merge29 : ltr: ae
+                -> l:s
+                -> atr:ae
+                -> a:s
+                -> btr:ae
+                -> b:s
+                -> Lemma (requires (sorted (tolist l) /\ sorted (tolist a) /\ sorted (tolist b) /\ (forall e. mem e ltr.l ==> not (member (get_id e) atr.l)) /\
+                              (forall e. mem e ltr.l ==> not (member (get_id e) btr.l)) /\
+                              (forall e. mem e atr.l ==> not (member (get_id e) btr.l)) /\
+                              (forall e e1. (memq e a /\ memq e1 l /\ (fst e = fst e1)) ==> (snd e = snd e1)) /\
+                              (forall e e1. (memq e b /\ memq e1 l /\ (fst e = fst e1)) ==> (snd e = snd e1)) /\
+                              (forall e e1. memq e l /\ mem e1 (diff_s (tolist a) (tolist l)) ==> fst e < fst e1) /\
+                              (forall e e1. memq e l /\ mem e1 (diff_s (tolist b) (tolist l)) ==> fst e < fst e1) /\
+                            (forall e e1. mem e (tolist l) /\ mem e1 (tolist l) /\ mem e (tolist a) /\ mem e1 (tolist a) /\ order e e1 (tolist l) ==> order e e1 (tolist a)) /\
+                            (forall e e1. mem e (tolist l) /\ mem e1 (tolist l) /\ mem e (tolist b) /\ mem e1 (tolist b) /\ order e e1 (tolist l) ==> order e e1 (tolist b)) /\
+                              (forall e e1. (mem e ltr.l /\ mem e1 atr.l ==> get_id e < get_id e1)) /\
+                              (forall e e1. (mem e ltr.l /\ mem e1 btr.l ==> get_id e < get_id e1)) /\
+                              (sim ltr l /\ sim (union ltr atr) a /\ sim (union ltr btr) b) /\
+                              (forall e. mem_id e (diff_s (tolist a) (tolist l)) ==> not (mem_id e (diff_s (tolist b) (tolist l)))) /\
+                              (forall e. mem_id e (diff_s (tolist b) (tolist l)) ==> not (mem_id e (diff_s (tolist a) (tolist l))))) /\
+                              (sim0 (absmerge ltr atr btr) (merge ltr l atr a btr b)))
+                       (ensures (forall e e1. mem e (filter_op (fun x -> is_enqueue x && mem x ltr.l && not
+                             (exists_mem ltr.l (fun d -> is_dequeue d && mem d ltr.l && mem x ltr.l && get_id x <> get_id d && matched x d ltr))
+                               && not (exists_mem (union ltr atr).l (fun d -> is_dequeue d && mem d (union ltr atr).l && mem x (union ltr atr).l &&
+                                         get_id x <> get_id d && matched x d (union ltr atr)))
+                               && not (exists_mem (union ltr btr).l (fun d -> is_dequeue d && mem d (union ltr btr).l && mem x (union ltr btr).l &&
+                                         get_id x <> get_id d && matched x d (union ltr btr)))) ltr.l) /\
+                               mem e1 (filter_op (fun x -> is_enqueue x && mem x atr.l && not
+                             (exists_mem atr.l (fun d -> is_dequeue d && mem d atr.l && mem x atr.l && get_id x <> get_id d && matched x d atr))) atr.l) /\
+                               get_id e <> get_id e1 /\ mem e1
+                             (filter_op (fun e1 -> get_id e <> get_id e1 && ((absmerge ltr atr btr).vis e e1)) (filter_op (fun x ->
+                               is_enqueue x && mem x (absmerge ltr atr btr).l && not
+                             (exists_mem (absmerge ltr atr btr).l (fun d -> is_dequeue d && mem d (absmerge ltr atr btr).l && mem x (absmerge ltr atr btr).l &&
+                               get_id x <> get_id d && matched x d (absmerge ltr atr btr)))) (absmerge ltr atr btr).l)) ==>
+                          (memq ((get_id e), (get_ele e)) (merge ltr l atr a btr b) /\ memq ((get_id e1), (get_ele e1)) (merge ltr l atr a btr b) /\
+                                get_id e <> get_id e1 /\ order ((get_id e), (get_ele e)) ((get_id e1), (get_ele e1)) (tolist (merge ltr l atr a btr b))
+                                      )))
+
+let prop_merge29 ltr l atr a btr b =
+  axiom_ae ltr; axiom_ae atr; axiom_ae btr; axiom_ae (union ltr atr); axiom_ae (union ltr btr);
+  prop_merge01 ltr l atr a btr b; prop_merge001 ltr l atr a btr b; prop_merge002 ltr l atr a btr b; prop_merge0 ltr l atr a btr b;
+  let tr = absmerge ltr atr btr in
+  let s0 = merge ltr l atr a btr b in
+  let enq_list = filter_op (fun x -> is_enqueue x && mem x tr.l && not
+                             (exists_mem tr.l (fun d -> is_dequeue d && mem d tr.l && mem x tr.l && get_id x <> get_id d && matched x d tr))) tr.l in
+
+  let enq_list4 = filter_op (fun x -> is_enqueue x && mem x atr.l && not
+                             (exists_mem atr.l (fun d -> is_dequeue d && mem d atr.l && mem x atr.l && get_id x <> get_id d && matched x d atr))) atr.l in
 
   let enq_list6 = filter_op (fun x -> is_enqueue x && mem x ltr.l && not
                              (exists_mem ltr.l (fun d -> is_dequeue d && mem d ltr.l && mem x ltr.l && get_id x <> get_id d && matched x d ltr))
@@ -1328,18 +1783,599 @@ let prop_merge1 ltr l atr a btr b =
                                && not (exists_mem (union ltr btr).l (fun d -> is_dequeue d && mem d (union ltr btr).l && mem x (union ltr btr).l &&
                                          get_id x <> get_id d && matched x d (union ltr btr)))) ltr.l in
 
-  // assert(forall e e1. mem e (tolist l) /\ mem e (tolist a) /\ mem e (tolist b) /\ mem e1 (tolist l) /\ mem e1 (tolist a) /\ mem e1 (tolist b) /\
-  //          (mem e1 (filter_s (fun e1 -> fst e <> fst e1 && order e e1 (intersection (tolist l) (tolist a) (tolist b)))
-  //                  (intersection (tolist l) (tolist a) (tolist b)))) ==>
-  //                   (mem (fst e, Enqueue (snd e)) (enq_list) && mem (fst e1, Enqueue (snd e1)) (enq_list6) && fst e <> fst e1 &&
-  //                      ((tr.vis (fst e, Enqueue (snd e)) (fst e1, Enqueue (snd e1))) ||
-  //                        (not (tr.vis (fst e, Enqueue (snd e)) (fst e1, Enqueue (snd e1)) ||
-  //                               tr.vis (fst e1, Enqueue (snd e1)) (fst e, Enqueue (snd e))) &&
-  //                  (fst e < fst e1)))
-  //          ));
-  admit(); ()
+  assert(forall e e1. mem e (enq_list6) /\ mem e1 (enq_list4) /\ get_id e <> get_id e1 /\ mem e1
+           (filter_op (fun e1 -> get_id e <> get_id e1 && (tr.vis e e1)) (enq_list)) ==>
+                          (memq ((get_id e), (get_ele e)) s0 /\ memq ((get_id e1), (get_ele e1)) s0 /\ get_id e <> get_id e1 /\
+                                      order ((get_id e), (get_ele e)) ((get_id e1), (get_ele e1)) (tolist s0)
+                                      ));
 
-#set-options "--initial_fuel 10 --ifuel 10 --initial_ifuel 10 --fuel 10 --z3rlimit 1000000"
+  ()
+
+val prop_merge210 : ltr: ae
+                -> l:s
+                -> atr:ae
+                -> a:s
+                -> btr:ae
+                -> b:s
+                -> Lemma (requires (sorted (tolist l) /\ sorted (tolist a) /\ sorted (tolist b) /\ (forall e. mem e ltr.l ==> not (member (get_id e) atr.l)) /\
+                              (forall e. mem e ltr.l ==> not (member (get_id e) btr.l)) /\
+                              (forall e. mem e atr.l ==> not (member (get_id e) btr.l)) /\
+                              (forall e e1. (memq e a /\ memq e1 l /\ (fst e = fst e1)) ==> (snd e = snd e1)) /\
+                              (forall e e1. (memq e b /\ memq e1 l /\ (fst e = fst e1)) ==> (snd e = snd e1)) /\
+                              (forall e e1. memq e l /\ mem e1 (diff_s (tolist a) (tolist l)) ==> fst e < fst e1) /\
+                              (forall e e1. memq e l /\ mem e1 (diff_s (tolist b) (tolist l)) ==> fst e < fst e1) /\
+                            (forall e e1. mem e (tolist l) /\ mem e1 (tolist l) /\ mem e (tolist a) /\ mem e1 (tolist a) /\ order e e1 (tolist l) ==> order e e1 (tolist a)) /\
+                            (forall e e1. mem e (tolist l) /\ mem e1 (tolist l) /\ mem e (tolist b) /\ mem e1 (tolist b) /\ order e e1 (tolist l) ==> order e e1 (tolist b)) /\
+                              (forall e e1. (mem e ltr.l /\ mem e1 atr.l ==> get_id e < get_id e1)) /\
+                              (forall e e1. (mem e ltr.l /\ mem e1 btr.l ==> get_id e < get_id e1)) /\
+                              (sim ltr l /\ sim (union ltr atr) a /\ sim (union ltr btr) b) /\
+                              (forall e. mem_id e (diff_s (tolist a) (tolist l)) ==> not (mem_id e (diff_s (tolist b) (tolist l)))) /\
+                              (forall e. mem_id e (diff_s (tolist b) (tolist l)) ==> not (mem_id e (diff_s (tolist a) (tolist l))))) /\
+                              (sim0 (absmerge ltr atr btr) (merge ltr l atr a btr b)))
+                       (ensures (forall e e1. mem e (filter_op (fun x -> is_enqueue x && mem x ltr.l && not
+                             (exists_mem ltr.l (fun d -> is_dequeue d && mem d ltr.l && mem x ltr.l && get_id x <> get_id d && matched x d ltr))
+                               && not (exists_mem (union ltr atr).l (fun d -> is_dequeue d && mem d (union ltr atr).l && mem x (union ltr atr).l &&
+                                         get_id x <> get_id d && matched x d (union ltr atr)))
+                               && not (exists_mem (union ltr btr).l (fun d -> is_dequeue d && mem d (union ltr btr).l && mem x (union ltr btr).l &&
+                                         get_id x <> get_id d && matched x d (union ltr btr)))) ltr.l) /\
+                               mem e1 (filter_op (fun x -> is_enqueue x && mem x btr.l && not
+                             (exists_mem btr.l (fun d -> is_dequeue d && mem d btr.l && mem x btr.l && get_id x <> get_id d && matched x d btr))) btr.l) /\
+                               get_id e <> get_id e1 /\ mem e1
+                             (filter_op (fun e1 -> get_id e <> get_id e1 && ((absmerge ltr atr btr).vis e e1)) (filter_op (fun x ->
+                               is_enqueue x && mem x (absmerge ltr atr btr).l && not
+                             (exists_mem (absmerge ltr atr btr).l (fun d -> is_dequeue d && mem d (absmerge ltr atr btr).l && mem x (absmerge ltr atr btr).l &&
+                               get_id x <> get_id d && matched x d (absmerge ltr atr btr)))) (absmerge ltr atr btr).l)) ==>
+                          (memq ((get_id e), (get_ele e)) (merge ltr l atr a btr b) /\ memq ((get_id e1), (get_ele e1)) (merge ltr l atr a btr b) /\
+                                get_id e <> get_id e1 /\ order ((get_id e), (get_ele e)) ((get_id e1), (get_ele e1)) (tolist (merge ltr l atr a btr b))
+                                      )))
+
+let prop_merge210 ltr l atr a btr b =
+  axiom_ae ltr; axiom_ae atr; axiom_ae btr; axiom_ae (union ltr atr); axiom_ae (union ltr btr);
+  prop_merge01 ltr l atr a btr b; prop_merge001 ltr l atr a btr b; prop_merge002 ltr l atr a btr b; prop_merge0 ltr l atr a btr b;
+  let tr = absmerge ltr atr btr in
+  let s0 = merge ltr l atr a btr b in
+  let enq_list = filter_op (fun x -> is_enqueue x && mem x tr.l && not
+                             (exists_mem tr.l (fun d -> is_dequeue d && mem d tr.l && mem x tr.l && get_id x <> get_id d && matched x d tr))) tr.l in
+
+  let enq_list5 = filter_op (fun x -> is_enqueue x && mem x btr.l && not
+                             (exists_mem btr.l (fun d -> is_dequeue d && mem d btr.l && mem x btr.l && get_id x <> get_id d && matched x d btr))) btr.l in
+
+  let enq_list6 = filter_op (fun x -> is_enqueue x && mem x ltr.l && not
+                             (exists_mem ltr.l (fun d -> is_dequeue d && mem d ltr.l && mem x ltr.l && get_id x <> get_id d && matched x d ltr))
+                               && not (exists_mem (union ltr atr).l (fun d -> is_dequeue d && mem d (union ltr atr).l && mem x (union ltr atr).l &&
+                                         get_id x <> get_id d && matched x d (union ltr atr)))
+                               && not (exists_mem (union ltr btr).l (fun d -> is_dequeue d && mem d (union ltr btr).l && mem x (union ltr btr).l &&
+                                         get_id x <> get_id d && matched x d (union ltr btr)))) ltr.l in
+
+  assert(forall e e1. mem e (enq_list6) /\ mem e1 (enq_list5) /\ get_id e <> get_id e1 /\ mem e1
+           (filter_op (fun e1 -> get_id e <> get_id e1 && ((tr.vis e e1))) (enq_list)) ==>
+                          (memq ((get_id e), (get_ele e)) s0 /\ memq ((get_id e1), (get_ele e1)) s0 /\ get_id e <> get_id e1 /\
+                                      order ((get_id e), (get_ele e)) ((get_id e1), (get_ele e1)) (tolist s0)
+                                      ));
+
+  ()
+
+val prop_merge211 : ltr: ae
+                -> l:s
+                -> atr:ae
+                -> a:s
+                -> btr:ae
+                -> b:s
+                -> Lemma (requires (sorted (tolist l) /\ sorted (tolist a) /\ sorted (tolist b) /\ (forall e. mem e ltr.l ==> not (member (get_id e) atr.l)) /\
+                              (forall e. mem e ltr.l ==> not (member (get_id e) btr.l)) /\
+                              (forall e. mem e atr.l ==> not (member (get_id e) btr.l)) /\
+                              (forall e e1. (memq e a /\ memq e1 l /\ (fst e = fst e1)) ==> (snd e = snd e1)) /\
+                              (forall e e1. (memq e b /\ memq e1 l /\ (fst e = fst e1)) ==> (snd e = snd e1)) /\
+                              (forall e e1. memq e l /\ mem e1 (diff_s (tolist a) (tolist l)) ==> fst e < fst e1) /\
+                              (forall e e1. memq e l /\ mem e1 (diff_s (tolist b) (tolist l)) ==> fst e < fst e1) /\
+                            (forall e e1. mem e (tolist l) /\ mem e1 (tolist l) /\ mem e (tolist a) /\ mem e1 (tolist a) /\ order e e1 (tolist l) ==> order e e1 (tolist a)) /\
+                            (forall e e1. mem e (tolist l) /\ mem e1 (tolist l) /\ mem e (tolist b) /\ mem e1 (tolist b) /\ order e e1 (tolist l) ==> order e e1 (tolist b)) /\
+                              (forall e e1. (mem e ltr.l /\ mem e1 atr.l ==> get_id e < get_id e1)) /\
+                              (forall e e1. (mem e ltr.l /\ mem e1 btr.l ==> get_id e < get_id e1)) /\
+                              (sim ltr l /\ sim (union ltr atr) a /\ sim (union ltr btr) b) /\
+                              (forall e. mem_id e (diff_s (tolist a) (tolist l)) ==> not (mem_id e (diff_s (tolist b) (tolist l)))) /\
+                              (forall e. mem_id e (diff_s (tolist b) (tolist l)) ==> not (mem_id e (diff_s (tolist a) (tolist l))))) /\
+                              (sim0 (absmerge ltr atr btr) (merge ltr l atr a btr b)))
+                       (ensures (forall e e1. mem e (filter_op (fun x -> is_enqueue x && mem x btr.l && not
+                             (exists_mem btr.l (fun d -> is_dequeue d && mem d btr.l && mem x btr.l && get_id x <> get_id d && matched x d btr))) btr.l) /\
+                               mem e1 (filter_op (fun x -> is_enqueue x && mem x ltr.l && not
+                             (exists_mem ltr.l (fun d -> is_dequeue d && mem d ltr.l && mem x ltr.l && get_id x <> get_id d && matched x d ltr))
+                               && not (exists_mem (union ltr atr).l (fun d -> is_dequeue d && mem d (union ltr atr).l && mem x (union ltr atr).l &&
+                                         get_id x <> get_id d && matched x d (union ltr atr)))
+                               && not (exists_mem (union ltr btr).l (fun d -> is_dequeue d && mem d (union ltr btr).l && mem x (union ltr btr).l &&
+                                         get_id x <> get_id d && matched x d (union ltr btr)))) ltr.l) /\
+                               get_id e <> get_id e1 /\ mem e1
+                             (filter_op (fun e1 -> get_id e <> get_id e1 && ((not ((absmerge ltr atr btr).vis e e1 ||
+                               (absmerge ltr atr btr).vis e1 e) && (get_id e < get_id e1)))) (filter_op (fun x ->
+                               is_enqueue x && mem x (absmerge ltr atr btr).l && not
+                             (exists_mem (absmerge ltr atr btr).l (fun d -> is_dequeue d && mem d (absmerge ltr atr btr).l && mem x (absmerge ltr atr btr).l &&
+                               get_id x <> get_id d && matched x d (absmerge ltr atr btr)))) (absmerge ltr atr btr).l)) ==>
+                          (memq ((get_id e), (get_ele e)) (merge ltr l atr a btr b) /\ memq ((get_id e1), (get_ele e1)) (merge ltr l atr a btr b) /\
+                                get_id e <> get_id e1 /\ order ((get_id e), (get_ele e)) ((get_id e1), (get_ele e1)) (tolist (merge ltr l atr a btr b))
+                                      )))
+
+let prop_merge211 ltr l atr a btr b =
+  axiom_ae ltr; axiom_ae atr; axiom_ae btr; axiom_ae (union ltr atr); axiom_ae (union ltr btr);
+  prop_merge01 ltr l atr a btr b; prop_merge001 ltr l atr a btr b; prop_merge002 ltr l atr a btr b; prop_merge0 ltr l atr a btr b;
+  let tr = absmerge ltr atr btr in
+  let s0 = merge ltr l atr a btr b in
+  let enq_list = filter_op (fun x -> is_enqueue x && mem x tr.l && not
+                             (exists_mem tr.l (fun d -> is_dequeue d && mem d tr.l && mem x tr.l && get_id x <> get_id d && matched x d tr))) tr.l in
+
+  let enq_list5 = filter_op (fun x -> is_enqueue x && mem x btr.l && not
+                             (exists_mem btr.l (fun d -> is_dequeue d && mem d btr.l && mem x btr.l && get_id x <> get_id d && matched x d btr))) btr.l in
+
+  let enq_list6 = filter_op (fun x -> is_enqueue x && mem x ltr.l && not
+                             (exists_mem ltr.l (fun d -> is_dequeue d && mem d ltr.l && mem x ltr.l && get_id x <> get_id d && matched x d ltr))
+                               && not (exists_mem (union ltr atr).l (fun d -> is_dequeue d && mem d (union ltr atr).l && mem x (union ltr atr).l &&
+                                         get_id x <> get_id d && matched x d (union ltr atr)))
+                               && not (exists_mem (union ltr btr).l (fun d -> is_dequeue d && mem d (union ltr btr).l && mem x (union ltr btr).l &&
+                                         get_id x <> get_id d && matched x d (union ltr btr)))) ltr.l in
+
+  assert(forall e e1. mem e (enq_list5) /\ mem e1 (enq_list6) /\ get_id e <> get_id e1 /\ mem e1
+           (filter_op (fun e1 -> get_id e <> get_id e1 && ((not (tr.vis e e1 || tr.vis e1 e) && (get_id e < get_id e1)))) (enq_list)) ==>
+                          (memq ((get_id e), (get_ele e)) s0 /\ memq ((get_id e1), (get_ele e1)) s0 /\ get_id e <> get_id e1 /\
+                                      order ((get_id e), (get_ele e)) ((get_id e1), (get_ele e1)) (tolist s0)
+                                      ));
+
+  ()
+
+val prop_merge212 : ltr: ae
+                -> l:s
+                -> atr:ae
+                -> a:s
+                -> btr:ae
+                -> b:s
+                -> Lemma (requires (sorted (tolist l) /\ sorted (tolist a) /\ sorted (tolist b) /\ (forall e. mem e ltr.l ==> not (member (get_id e) atr.l)) /\
+                              (forall e. mem e ltr.l ==> not (member (get_id e) btr.l)) /\
+                              (forall e. mem e atr.l ==> not (member (get_id e) btr.l)) /\
+                              (forall e e1. (memq e a /\ memq e1 l /\ (fst e = fst e1)) ==> (snd e = snd e1)) /\
+                              (forall e e1. (memq e b /\ memq e1 l /\ (fst e = fst e1)) ==> (snd e = snd e1)) /\
+                              (forall e e1. memq e l /\ mem e1 (diff_s (tolist a) (tolist l)) ==> fst e < fst e1) /\
+                              (forall e e1. memq e l /\ mem e1 (diff_s (tolist b) (tolist l)) ==> fst e < fst e1) /\
+                            (forall e e1. mem e (tolist l) /\ mem e1 (tolist l) /\ mem e (tolist a) /\ mem e1 (tolist a) /\ order e e1 (tolist l) ==> order e e1 (tolist a)) /\
+                            (forall e e1. mem e (tolist l) /\ mem e1 (tolist l) /\ mem e (tolist b) /\ mem e1 (tolist b) /\ order e e1 (tolist l) ==> order e e1 (tolist b)) /\
+                              (forall e e1. (mem e ltr.l /\ mem e1 atr.l ==> get_id e < get_id e1)) /\
+                              (forall e e1. (mem e ltr.l /\ mem e1 btr.l ==> get_id e < get_id e1)) /\
+                              (sim ltr l /\ sim (union ltr atr) a /\ sim (union ltr btr) b) /\
+                              (forall e. mem_id e (diff_s (tolist a) (tolist l)) ==> not (mem_id e (diff_s (tolist b) (tolist l)))) /\
+                              (forall e. mem_id e (diff_s (tolist b) (tolist l)) ==> not (mem_id e (diff_s (tolist a) (tolist l))))) /\
+                              (sim0 (absmerge ltr atr btr) (merge ltr l atr a btr b)))
+                       (ensures (forall e e1. mem e (filter_op (fun x -> is_enqueue x && mem x atr.l && not
+                             (exists_mem atr.l (fun d -> is_dequeue d && mem d atr.l && mem x atr.l && get_id x <> get_id d && matched x d atr))) atr.l) /\
+                               mem e1 (filter_op (fun x -> is_enqueue x && mem x ltr.l && not
+                             (exists_mem ltr.l (fun d -> is_dequeue d && mem d ltr.l && mem x ltr.l && get_id x <> get_id d && matched x d ltr))
+                               && not (exists_mem (union ltr atr).l (fun d -> is_dequeue d && mem d (union ltr atr).l && mem x (union ltr atr).l &&
+                                         get_id x <> get_id d && matched x d (union ltr atr)))
+                               && not (exists_mem (union ltr btr).l (fun d -> is_dequeue d && mem d (union ltr btr).l && mem x (union ltr btr).l &&
+                                         get_id x <> get_id d && matched x d (union ltr btr)))) ltr.l) /\
+                               get_id e <> get_id e1 /\ mem e1
+                             (filter_op (fun e1 -> get_id e <> get_id e1 && ((not ((absmerge ltr atr btr).vis e e1 ||
+                               (absmerge ltr atr btr).vis e1 e) && (get_id e < get_id e1)))) (filter_op (fun x ->
+                               is_enqueue x && mem x (absmerge ltr atr btr).l && not
+                             (exists_mem (absmerge ltr atr btr).l (fun d -> is_dequeue d && mem d (absmerge ltr atr btr).l && mem x (absmerge ltr atr btr).l &&
+                               get_id x <> get_id d && matched x d (absmerge ltr atr btr)))) (absmerge ltr atr btr).l)) ==>
+                          (memq ((get_id e), (get_ele e)) (merge ltr l atr a btr b) /\ memq ((get_id e1), (get_ele e1)) (merge ltr l atr a btr b) /\
+                                get_id e <> get_id e1 /\ order ((get_id e), (get_ele e)) ((get_id e1), (get_ele e1)) (tolist (merge ltr l atr a btr b))
+                                      )))
+
+let prop_merge212 ltr l atr a btr b =
+  axiom_ae ltr; axiom_ae atr; axiom_ae btr; axiom_ae (union ltr atr); axiom_ae (union ltr btr);
+  prop_merge01 ltr l atr a btr b; prop_merge001 ltr l atr a btr b; prop_merge002 ltr l atr a btr b; prop_merge0 ltr l atr a btr b;
+  let tr = absmerge ltr atr btr in
+  let s0 = merge ltr l atr a btr b in
+  let enq_list = filter_op (fun x -> is_enqueue x && mem x tr.l && not
+                             (exists_mem tr.l (fun d -> is_dequeue d && mem d tr.l && mem x tr.l && get_id x <> get_id d && matched x d tr))) tr.l in
+
+  let enq_list4 = filter_op (fun x -> is_enqueue x && mem x atr.l && not
+                             (exists_mem atr.l (fun d -> is_dequeue d && mem d atr.l && mem x atr.l && get_id x <> get_id d && matched x d atr))) atr.l in
+
+  let enq_list6 = filter_op (fun x -> is_enqueue x && mem x ltr.l && not
+                             (exists_mem ltr.l (fun d -> is_dequeue d && mem d ltr.l && mem x ltr.l && get_id x <> get_id d && matched x d ltr))
+                               && not (exists_mem (union ltr atr).l (fun d -> is_dequeue d && mem d (union ltr atr).l && mem x (union ltr atr).l &&
+                                         get_id x <> get_id d && matched x d (union ltr atr)))
+                               && not (exists_mem (union ltr btr).l (fun d -> is_dequeue d && mem d (union ltr btr).l && mem x (union ltr btr).l &&
+                                         get_id x <> get_id d && matched x d (union ltr btr)))) ltr.l in
+
+  assert(forall e e1. mem e (enq_list4) /\ mem e1 (enq_list6) /\ get_id e <> get_id e1 /\ mem e1
+           (filter_op (fun e1 -> get_id e <> get_id e1 && ((not (tr.vis e e1 || tr.vis e1 e) && (get_id e < get_id e1)))) (enq_list)) ==>
+                          (memq ((get_id e), (get_ele e)) s0 /\ memq ((get_id e1), (get_ele e1)) s0 /\ get_id e <> get_id e1 /\
+                                      order ((get_id e), (get_ele e)) ((get_id e1), (get_ele e1)) (tolist s0)
+                                      ));
+
+  ()
+
+
+val prop_merge213 : ltr: ae
+                -> l:s
+                -> atr:ae
+                -> a:s
+                -> btr:ae
+                -> b:s
+                -> Lemma (requires (sorted (tolist l) /\ sorted (tolist a) /\ sorted (tolist b) /\ (forall e. mem e ltr.l ==> not (member (get_id e) atr.l)) /\
+                              (forall e. mem e ltr.l ==> not (member (get_id e) btr.l)) /\
+                              (forall e. mem e atr.l ==> not (member (get_id e) btr.l)) /\
+                              (forall e e1. (memq e a /\ memq e1 l /\ (fst e = fst e1)) ==> (snd e = snd e1)) /\
+                              (forall e e1. (memq e b /\ memq e1 l /\ (fst e = fst e1)) ==> (snd e = snd e1)) /\
+                              (forall e e1. memq e l /\ mem e1 (diff_s (tolist a) (tolist l)) ==> fst e < fst e1) /\
+                              (forall e e1. memq e l /\ mem e1 (diff_s (tolist b) (tolist l)) ==> fst e < fst e1) /\
+                            (forall e e1. mem e (tolist l) /\ mem e1 (tolist l) /\ mem e (tolist a) /\ mem e1 (tolist a) /\ order e e1 (tolist l) ==> order e e1 (tolist a)) /\
+                            (forall e e1. mem e (tolist l) /\ mem e1 (tolist l) /\ mem e (tolist b) /\ mem e1 (tolist b) /\ order e e1 (tolist l) ==> order e e1 (tolist b)) /\
+                              (forall e e1. (mem e ltr.l /\ mem e1 atr.l ==> get_id e < get_id e1)) /\
+                              (forall e e1. (mem e ltr.l /\ mem e1 btr.l ==> get_id e < get_id e1)) /\
+                              (sim ltr l /\ sim (union ltr atr) a /\ sim (union ltr btr) b) /\
+                              (forall e. mem_id e (diff_s (tolist a) (tolist l)) ==> not (mem_id e (diff_s (tolist b) (tolist l)))) /\
+                              (forall e. mem_id e (diff_s (tolist b) (tolist l)) ==> not (mem_id e (diff_s (tolist a) (tolist l))))) /\
+                              (sim0 (absmerge ltr atr btr) (merge ltr l atr a btr b)))
+                       (ensures (forall e e1. mem e (filter_op (fun x -> is_enqueue x && mem x btr.l && not
+                             (exists_mem btr.l (fun d -> is_dequeue d && mem d btr.l && mem x btr.l && get_id x <> get_id d && matched x d btr))) btr.l) /\
+                               mem e1 (filter_op (fun x -> is_enqueue x && mem x ltr.l && not
+                             (exists_mem ltr.l (fun d -> is_dequeue d && mem d ltr.l && mem x ltr.l && get_id x <> get_id d && matched x d ltr))
+                               && not (exists_mem (union ltr atr).l (fun d -> is_dequeue d && mem d (union ltr atr).l && mem x (union ltr atr).l &&
+                                         get_id x <> get_id d && matched x d (union ltr atr)))
+                               && not (exists_mem (union ltr btr).l (fun d -> is_dequeue d && mem d (union ltr btr).l && mem x (union ltr btr).l &&
+                                         get_id x <> get_id d && matched x d (union ltr btr)))) ltr.l) /\
+                               get_id e <> get_id e1 /\ mem e1
+                             (filter_op (fun e1 -> get_id e <> get_id e1 && ((absmerge ltr atr btr).vis e e1)) (filter_op (fun x ->
+                               is_enqueue x && mem x (absmerge ltr atr btr).l && not
+                             (exists_mem (absmerge ltr atr btr).l (fun d -> is_dequeue d && mem d (absmerge ltr atr btr).l && mem x (absmerge ltr atr btr).l &&
+                               get_id x <> get_id d && matched x d (absmerge ltr atr btr)))) (absmerge ltr atr btr).l)) ==>
+                          (memq ((get_id e), (get_ele e)) (merge ltr l atr a btr b) /\ memq ((get_id e1), (get_ele e1)) (merge ltr l atr a btr b) /\
+                                get_id e <> get_id e1 /\ order ((get_id e), (get_ele e)) ((get_id e1), (get_ele e1)) (tolist (merge ltr l atr a btr b))
+                                      )))
+
+let prop_merge213 ltr l atr a btr b =
+  axiom_ae ltr; axiom_ae atr; axiom_ae btr; axiom_ae (union ltr atr); axiom_ae (union ltr btr);
+  prop_merge01 ltr l atr a btr b; prop_merge001 ltr l atr a btr b; prop_merge002 ltr l atr a btr b; prop_merge0 ltr l atr a btr b;
+  let tr = absmerge ltr atr btr in
+  let s0 = merge ltr l atr a btr b in
+  let enq_list = filter_op (fun x -> is_enqueue x && mem x tr.l && not
+                             (exists_mem tr.l (fun d -> is_dequeue d && mem d tr.l && mem x tr.l && get_id x <> get_id d && matched x d tr))) tr.l in
+
+  let enq_list5 = filter_op (fun x -> is_enqueue x && mem x btr.l && not
+                             (exists_mem btr.l (fun d -> is_dequeue d && mem d btr.l && mem x btr.l && get_id x <> get_id d && matched x d btr))) btr.l in
+
+  let enq_list6 = filter_op (fun x -> is_enqueue x && mem x ltr.l && not
+                             (exists_mem ltr.l (fun d -> is_dequeue d && mem d ltr.l && mem x ltr.l && get_id x <> get_id d && matched x d ltr))
+                               && not (exists_mem (union ltr atr).l (fun d -> is_dequeue d && mem d (union ltr atr).l && mem x (union ltr atr).l &&
+                                         get_id x <> get_id d && matched x d (union ltr atr)))
+                               && not (exists_mem (union ltr btr).l (fun d -> is_dequeue d && mem d (union ltr btr).l && mem x (union ltr btr).l &&
+                                         get_id x <> get_id d && matched x d (union ltr btr)))) ltr.l in
+
+  assert(forall e e1. mem e (enq_list5) /\ mem e1 (enq_list6) /\ get_id e <> get_id e1 /\ mem e1
+           (filter_op (fun e1 -> get_id e <> get_id e1 && (tr.vis e e1)) (enq_list)) ==>
+                          (memq ((get_id e), (get_ele e)) s0 /\ memq ((get_id e1), (get_ele e1)) s0 /\ get_id e <> get_id e1 /\
+                                      order ((get_id e), (get_ele e)) ((get_id e1), (get_ele e1)) (tolist s0)
+                                      ));
+
+  ()
+
+val prop_merge214 : ltr: ae
+                -> l:s
+                -> atr:ae
+                -> a:s
+                -> btr:ae
+                -> b:s
+                -> Lemma (requires (sorted (tolist l) /\ sorted (tolist a) /\ sorted (tolist b) /\ (forall e. mem e ltr.l ==> not (member (get_id e) atr.l)) /\
+                              (forall e. mem e ltr.l ==> not (member (get_id e) btr.l)) /\
+                              (forall e. mem e atr.l ==> not (member (get_id e) btr.l)) /\
+                              (forall e e1. (memq e a /\ memq e1 l /\ (fst e = fst e1)) ==> (snd e = snd e1)) /\
+                              (forall e e1. (memq e b /\ memq e1 l /\ (fst e = fst e1)) ==> (snd e = snd e1)) /\
+                              (forall e e1. memq e l /\ mem e1 (diff_s (tolist a) (tolist l)) ==> fst e < fst e1) /\
+                              (forall e e1. memq e l /\ mem e1 (diff_s (tolist b) (tolist l)) ==> fst e < fst e1) /\
+                            (forall e e1. mem e (tolist l) /\ mem e1 (tolist l) /\ mem e (tolist a) /\ mem e1 (tolist a) /\ order e e1 (tolist l) ==> order e e1 (tolist a)) /\
+                            (forall e e1. mem e (tolist l) /\ mem e1 (tolist l) /\ mem e (tolist b) /\ mem e1 (tolist b) /\ order e e1 (tolist l) ==> order e e1 (tolist b)) /\
+                              (forall e e1. (mem e ltr.l /\ mem e1 atr.l ==> get_id e < get_id e1)) /\
+                              (forall e e1. (mem e ltr.l /\ mem e1 btr.l ==> get_id e < get_id e1)) /\
+                              (sim ltr l /\ sim (union ltr atr) a /\ sim (union ltr btr) b) /\
+                              (forall e. mem_id e (diff_s (tolist a) (tolist l)) ==> not (mem_id e (diff_s (tolist b) (tolist l)))) /\
+                              (forall e. mem_id e (diff_s (tolist b) (tolist l)) ==> not (mem_id e (diff_s (tolist a) (tolist l))))) /\
+                              (sim0 (absmerge ltr atr btr) (merge ltr l atr a btr b)))
+                       (ensures (forall e e1. mem e (filter_op (fun x -> is_enqueue x && mem x atr.l && not
+                             (exists_mem atr.l (fun d -> is_dequeue d && mem d atr.l && mem x atr.l && get_id x <> get_id d && matched x d atr))) atr.l) /\
+                               mem e1 (filter_op (fun x -> is_enqueue x && mem x ltr.l && not
+                             (exists_mem ltr.l (fun d -> is_dequeue d && mem d ltr.l && mem x ltr.l && get_id x <> get_id d && matched x d ltr))
+                               && not (exists_mem (union ltr atr).l (fun d -> is_dequeue d && mem d (union ltr atr).l && mem x (union ltr atr).l &&
+                                         get_id x <> get_id d && matched x d (union ltr atr)))
+                               && not (exists_mem (union ltr btr).l (fun d -> is_dequeue d && mem d (union ltr btr).l && mem x (union ltr btr).l &&
+                                         get_id x <> get_id d && matched x d (union ltr btr)))) ltr.l) /\
+                               get_id e <> get_id e1 /\ mem e1
+                             (filter_op (fun e1 -> get_id e <> get_id e1 && ((absmerge ltr atr btr).vis e e1)) (filter_op (fun x ->
+                               is_enqueue x && mem x (absmerge ltr atr btr).l && not
+                             (exists_mem (absmerge ltr atr btr).l (fun d -> is_dequeue d && mem d (absmerge ltr atr btr).l && mem x (absmerge ltr atr btr).l &&
+                               get_id x <> get_id d && matched x d (absmerge ltr atr btr)))) (absmerge ltr atr btr).l)) ==>
+                          (memq ((get_id e), (get_ele e)) (merge ltr l atr a btr b) /\ memq ((get_id e1), (get_ele e1)) (merge ltr l atr a btr b) /\
+                                get_id e <> get_id e1 /\ order ((get_id e), (get_ele e)) ((get_id e1), (get_ele e1)) (tolist (merge ltr l atr a btr b))
+                                      )))
+
+let prop_merge214 ltr l atr a btr b =
+  axiom_ae ltr; axiom_ae atr; axiom_ae btr; axiom_ae (union ltr atr); axiom_ae (union ltr btr);
+  prop_merge01 ltr l atr a btr b; prop_merge001 ltr l atr a btr b; prop_merge002 ltr l atr a btr b; prop_merge0 ltr l atr a btr b;
+  let tr = absmerge ltr atr btr in
+  let s0 = merge ltr l atr a btr b in
+  let enq_list = filter_op (fun x -> is_enqueue x && mem x tr.l && not
+                             (exists_mem tr.l (fun d -> is_dequeue d && mem d tr.l && mem x tr.l && get_id x <> get_id d && matched x d tr))) tr.l in
+
+  let enq_list4 = filter_op (fun x -> is_enqueue x && mem x atr.l && not
+                             (exists_mem atr.l (fun d -> is_dequeue d && mem d atr.l && mem x atr.l && get_id x <> get_id d && matched x d atr))) atr.l in
+
+  let enq_list6 = filter_op (fun x -> is_enqueue x && mem x ltr.l && not
+                             (exists_mem ltr.l (fun d -> is_dequeue d && mem d ltr.l && mem x ltr.l && get_id x <> get_id d && matched x d ltr))
+                               && not (exists_mem (union ltr atr).l (fun d -> is_dequeue d && mem d (union ltr atr).l && mem x (union ltr atr).l &&
+                                         get_id x <> get_id d && matched x d (union ltr atr)))
+                               && not (exists_mem (union ltr btr).l (fun d -> is_dequeue d && mem d (union ltr btr).l && mem x (union ltr btr).l &&
+                                         get_id x <> get_id d && matched x d (union ltr btr)))) ltr.l in
+
+  assert(forall e e1. mem e (enq_list4) /\ mem e1 (enq_list6) /\ get_id e <> get_id e1 /\ mem e1
+           (filter_op (fun e1 -> get_id e <> get_id e1 && ((tr.vis e e1))) (enq_list)) ==>
+                          (memq ((get_id e), (get_ele e)) s0 /\ memq ((get_id e1), (get_ele e1)) s0 /\ get_id e <> get_id e1 /\
+                                      order ((get_id e), (get_ele e)) ((get_id e1), (get_ele e1)) (tolist s0)
+                                      ));
+
+  ()
+
+val prop_merge215 : ltr: ae
+                -> l:s
+                -> atr:ae
+                -> a:s
+                -> btr:ae
+                -> b:s
+                -> Lemma (requires (sorted (tolist l) /\ sorted (tolist a) /\ sorted (tolist b) /\ (forall e. mem e ltr.l ==> not (member (get_id e) atr.l)) /\
+                              (forall e. mem e ltr.l ==> not (member (get_id e) btr.l)) /\
+                              (forall e. mem e atr.l ==> not (member (get_id e) btr.l)) /\
+                              (forall e e1. (memq e a /\ memq e1 l /\ (fst e = fst e1)) ==> (snd e = snd e1)) /\
+                              (forall e e1. (memq e b /\ memq e1 l /\ (fst e = fst e1)) ==> (snd e = snd e1)) /\
+                              (forall e e1. memq e l /\ mem e1 (diff_s (tolist a) (tolist l)) ==> fst e < fst e1) /\
+                              (forall e e1. memq e l /\ mem e1 (diff_s (tolist b) (tolist l)) ==> fst e < fst e1) /\
+                            (forall e e1. mem e (tolist l) /\ mem e1 (tolist l) /\ mem e (tolist a) /\ mem e1 (tolist a) /\ order e e1 (tolist l) ==> order e e1 (tolist a)) /\
+                            (forall e e1. mem e (tolist l) /\ mem e1 (tolist l) /\ mem e (tolist b) /\ mem e1 (tolist b) /\ order e e1 (tolist l) ==> order e e1 (tolist b)) /\
+                              (forall e e1. (mem e ltr.l /\ mem e1 atr.l ==> get_id e < get_id e1)) /\
+                              (forall e e1. (mem e ltr.l /\ mem e1 btr.l ==> get_id e < get_id e1)) /\
+                              (sim ltr l /\ sim (union ltr atr) a /\ sim (union ltr btr) b) /\
+                              (forall e. mem_id e (diff_s (tolist a) (tolist l)) ==> not (mem_id e (diff_s (tolist b) (tolist l)))) /\
+                              (forall e. mem_id e (diff_s (tolist b) (tolist l)) ==> not (mem_id e (diff_s (tolist a) (tolist l))))) /\
+                              (sim0 (absmerge ltr atr btr) (merge ltr l atr a btr b)))
+                       (ensures (forall e e1. mem e (filter_op (fun x -> is_enqueue x && mem x ltr.l && not
+                             (exists_mem ltr.l (fun d -> is_dequeue d && mem d ltr.l && mem x ltr.l && get_id x <> get_id d && matched x d ltr))
+                               && not (exists_mem (union ltr atr).l (fun d -> is_dequeue d && mem d (union ltr atr).l && mem x (union ltr atr).l &&
+                                         get_id x <> get_id d && matched x d (union ltr atr)))
+                               && not (exists_mem (union ltr btr).l (fun d -> is_dequeue d && mem d (union ltr btr).l && mem x (union ltr btr).l &&
+                                         get_id x <> get_id d && matched x d (union ltr btr)))) ltr.l) /\
+                               mem e1 (filter_op (fun x -> is_enqueue x && mem x btr.l && not
+                             (exists_mem btr.l (fun d -> is_dequeue d && mem d btr.l && mem x btr.l && get_id x <> get_id d && matched x d btr))) btr.l) /\
+                               get_id e <> get_id e1 /\ mem e1
+                             (filter_op (fun e1 -> get_id e <> get_id e1 && ((not ((absmerge ltr atr btr).vis e e1 ||
+                               (absmerge ltr atr btr).vis e1 e) && (get_id e < get_id e1)))) (filter_op (fun x ->
+                               is_enqueue x && mem x (absmerge ltr atr btr).l && not
+                             (exists_mem (absmerge ltr atr btr).l (fun d -> is_dequeue d && mem d (absmerge ltr atr btr).l && mem x (absmerge ltr atr btr).l &&
+                               get_id x <> get_id d && matched x d (absmerge ltr atr btr)))) (absmerge ltr atr btr).l)) ==>
+                          (memq ((get_id e), (get_ele e)) (merge ltr l atr a btr b) /\ memq ((get_id e1), (get_ele e1)) (merge ltr l atr a btr b) /\
+                                get_id e <> get_id e1 /\ order ((get_id e), (get_ele e)) ((get_id e1), (get_ele e1)) (tolist (merge ltr l atr a btr b))
+                                      )))
+
+let prop_merge215 ltr l atr a btr b =
+  axiom_ae ltr; axiom_ae atr; axiom_ae btr; axiom_ae (union ltr atr); axiom_ae (union ltr btr);
+  prop_merge01 ltr l atr a btr b; prop_merge001 ltr l atr a btr b; prop_merge002 ltr l atr a btr b; prop_merge0 ltr l atr a btr b;
+  let tr = absmerge ltr atr btr in
+  let s0 = merge ltr l atr a btr b in
+  let enq_list = filter_op (fun x -> is_enqueue x && mem x tr.l && not
+                             (exists_mem tr.l (fun d -> is_dequeue d && mem d tr.l && mem x tr.l && get_id x <> get_id d && matched x d tr))) tr.l in
+
+  let enq_list5 = filter_op (fun x -> is_enqueue x && mem x btr.l && not
+                             (exists_mem btr.l (fun d -> is_dequeue d && mem d btr.l && mem x btr.l && get_id x <> get_id d && matched x d btr))) btr.l in
+
+  let enq_list6 = filter_op (fun x -> is_enqueue x && mem x ltr.l && not
+                             (exists_mem ltr.l (fun d -> is_dequeue d && mem d ltr.l && mem x ltr.l && get_id x <> get_id d && matched x d ltr))
+                               && not (exists_mem (union ltr atr).l (fun d -> is_dequeue d && mem d (union ltr atr).l && mem x (union ltr atr).l &&
+                                         get_id x <> get_id d && matched x d (union ltr atr)))
+                               && not (exists_mem (union ltr btr).l (fun d -> is_dequeue d && mem d (union ltr btr).l && mem x (union ltr btr).l &&
+                                         get_id x <> get_id d && matched x d (union ltr btr)))) ltr.l in
+
+  assert(forall e e1. mem e (enq_list6) /\ mem e1 (enq_list5) /\ get_id e <> get_id e1 /\ mem e1
+           (filter_op (fun e1 -> get_id e <> get_id e1 && ((not (tr.vis e e1 || tr.vis e1 e) && (get_id e < get_id e1)))) (enq_list)) ==>
+                          (memq ((get_id e), (get_ele e)) s0 /\ memq ((get_id e1), (get_ele e1)) s0 /\ get_id e <> get_id e1 /\
+                                      order ((get_id e), (get_ele e)) ((get_id e1), (get_ele e1)) (tolist s0)
+                                      ));
+
+  ()
+
+val prop_merge216 : ltr: ae
+                -> l:s
+                -> atr:ae
+                -> a:s
+                -> btr:ae
+                -> b:s
+                -> Lemma (requires (sorted (tolist l) /\ sorted (tolist a) /\ sorted (tolist b) /\ (forall e. mem e ltr.l ==> not (member (get_id e) atr.l)) /\
+                              (forall e. mem e ltr.l ==> not (member (get_id e) btr.l)) /\
+                              (forall e. mem e atr.l ==> not (member (get_id e) btr.l)) /\
+                              (forall e e1. (memq e a /\ memq e1 l /\ (fst e = fst e1)) ==> (snd e = snd e1)) /\
+                              (forall e e1. (memq e b /\ memq e1 l /\ (fst e = fst e1)) ==> (snd e = snd e1)) /\
+                              (forall e e1. memq e l /\ mem e1 (diff_s (tolist a) (tolist l)) ==> fst e < fst e1) /\
+                              (forall e e1. memq e l /\ mem e1 (diff_s (tolist b) (tolist l)) ==> fst e < fst e1) /\
+                            (forall e e1. mem e (tolist l) /\ mem e1 (tolist l) /\ mem e (tolist a) /\ mem e1 (tolist a) /\ order e e1 (tolist l) ==> order e e1 (tolist a)) /\
+                            (forall e e1. mem e (tolist l) /\ mem e1 (tolist l) /\ mem e (tolist b) /\ mem e1 (tolist b) /\ order e e1 (tolist l) ==> order e e1 (tolist b)) /\
+                              (forall e e1. (mem e ltr.l /\ mem e1 atr.l ==> get_id e < get_id e1)) /\
+                              (forall e e1. (mem e ltr.l /\ mem e1 btr.l ==> get_id e < get_id e1)) /\
+                              (sim ltr l /\ sim (union ltr atr) a /\ sim (union ltr btr) b) /\
+                              (forall e. mem_id e (diff_s (tolist a) (tolist l)) ==> not (mem_id e (diff_s (tolist b) (tolist l)))) /\
+                              (forall e. mem_id e (diff_s (tolist b) (tolist l)) ==> not (mem_id e (diff_s (tolist a) (tolist l))))) /\
+                              (sim0 (absmerge ltr atr btr) (merge ltr l atr a btr b)))
+                       (ensures (forall e e1. mem e (filter_op (fun x -> is_enqueue x && mem x ltr.l && not
+                             (exists_mem ltr.l (fun d -> is_dequeue d && mem d ltr.l && mem x ltr.l && get_id x <> get_id d && matched x d ltr))
+                               && not (exists_mem (union ltr atr).l (fun d -> is_dequeue d && mem d (union ltr atr).l && mem x (union ltr atr).l &&
+                                         get_id x <> get_id d && matched x d (union ltr atr)))
+                               && not (exists_mem (union ltr btr).l (fun d -> is_dequeue d && mem d (union ltr btr).l && mem x (union ltr btr).l &&
+                                         get_id x <> get_id d && matched x d (union ltr btr)))) ltr.l) /\
+                               mem e1 (filter_op (fun x -> is_enqueue x && mem x atr.l && not
+                             (exists_mem atr.l (fun d -> is_dequeue d && mem d atr.l && mem x atr.l && get_id x <> get_id d && matched x d atr))) atr.l) /\
+                               get_id e <> get_id e1 /\ mem e1
+                             (filter_op (fun e1 -> get_id e <> get_id e1 && ((not ((absmerge ltr atr btr).vis e e1 ||
+                               (absmerge ltr atr btr).vis e1 e) && (get_id e < get_id e1)))) (filter_op (fun x ->
+                               is_enqueue x && mem x (absmerge ltr atr btr).l && not
+                             (exists_mem (absmerge ltr atr btr).l (fun d -> is_dequeue d && mem d (absmerge ltr atr btr).l && mem x (absmerge ltr atr btr).l &&
+                               get_id x <> get_id d && matched x d (absmerge ltr atr btr)))) (absmerge ltr atr btr).l)) ==>
+                          (memq ((get_id e), (get_ele e)) (merge ltr l atr a btr b) /\ memq ((get_id e1), (get_ele e1)) (merge ltr l atr a btr b) /\
+                                get_id e <> get_id e1 /\ order ((get_id e), (get_ele e)) ((get_id e1), (get_ele e1)) (tolist (merge ltr l atr a btr b))
+                                      )))
+
+let prop_merge216 ltr l atr a btr b =
+  axiom_ae ltr; axiom_ae atr; axiom_ae btr; axiom_ae (union ltr atr); axiom_ae (union ltr btr);
+  prop_merge01 ltr l atr a btr b; prop_merge001 ltr l atr a btr b; prop_merge002 ltr l atr a btr b; prop_merge0 ltr l atr a btr b;
+  let tr = absmerge ltr atr btr in
+  let s0 = merge ltr l atr a btr b in
+  let enq_list = filter_op (fun x -> is_enqueue x && mem x tr.l && not
+                             (exists_mem tr.l (fun d -> is_dequeue d && mem d tr.l && mem x tr.l && get_id x <> get_id d && matched x d tr))) tr.l in
+
+  let enq_list4 = filter_op (fun x -> is_enqueue x && mem x atr.l && not
+                             (exists_mem atr.l (fun d -> is_dequeue d && mem d atr.l && mem x atr.l && get_id x <> get_id d && matched x d atr))) atr.l in
+
+  let enq_list6 = filter_op (fun x -> is_enqueue x && mem x ltr.l && not
+                             (exists_mem ltr.l (fun d -> is_dequeue d && mem d ltr.l && mem x ltr.l && get_id x <> get_id d && matched x d ltr))
+                               && not (exists_mem (union ltr atr).l (fun d -> is_dequeue d && mem d (union ltr atr).l && mem x (union ltr atr).l &&
+                                         get_id x <> get_id d && matched x d (union ltr atr)))
+                               && not (exists_mem (union ltr btr).l (fun d -> is_dequeue d && mem d (union ltr btr).l && mem x (union ltr btr).l &&
+                                         get_id x <> get_id d && matched x d (union ltr btr)))) ltr.l in
+
+  assert(forall e e1. mem e (enq_list6) /\ mem e1 (enq_list4) /\ get_id e <> get_id e1 /\ mem e1
+           (filter_op (fun e1 -> get_id e <> get_id e1 && ((not (tr.vis e e1 || tr.vis e1 e) && (get_id e < get_id e1)))) (enq_list)) ==>
+                          (memq ((get_id e), (get_ele e)) s0 /\ memq ((get_id e1), (get_ele e1)) s0 /\ get_id e <> get_id e1 /\
+                                      order ((get_id e), (get_ele e)) ((get_id e1), (get_ele e1)) (tolist s0)
+                                      ));
+
+  ()
+
+val prop_merge218 : ltr: ae
+                -> l:s
+                -> atr:ae
+                -> a:s
+                -> btr:ae
+                -> b:s
+                -> Lemma (requires (sorted (tolist l) /\ sorted (tolist a) /\ sorted (tolist b) /\ (forall e. mem e ltr.l ==> not (member (get_id e) atr.l)) /\
+                              (forall e. mem e ltr.l ==> not (member (get_id e) btr.l)) /\
+                              (forall e. mem e atr.l ==> not (member (get_id e) btr.l)) /\
+                              (forall e e1. (memq e a /\ memq e1 l /\ (fst e = fst e1)) ==> (snd e = snd e1)) /\
+                              (forall e e1. (memq e b /\ memq e1 l /\ (fst e = fst e1)) ==> (snd e = snd e1)) /\
+                              (forall e e1. memq e l /\ mem e1 (diff_s (tolist a) (tolist l)) ==> fst e < fst e1) /\
+                              (forall e e1. memq e l /\ mem e1 (diff_s (tolist b) (tolist l)) ==> fst e < fst e1) /\
+                            (forall e e1. mem e (tolist l) /\ mem e1 (tolist l) /\ mem e (tolist a) /\ mem e1 (tolist a) /\ order e e1 (tolist l) ==> order e e1 (tolist a)) /\
+                            (forall e e1. mem e (tolist l) /\ mem e1 (tolist l) /\ mem e (tolist b) /\ mem e1 (tolist b) /\ order e e1 (tolist l) ==> order e e1 (tolist b)) /\
+                              (forall e e1. (mem e ltr.l /\ mem e1 atr.l ==> get_id e < get_id e1)) /\
+                              (forall e e1. (mem e ltr.l /\ mem e1 btr.l ==> get_id e < get_id e1)) /\
+                              (sim ltr l /\ sim (union ltr atr) a /\ sim (union ltr btr) b) /\
+                              (forall e. mem_id e (diff_s (tolist a) (tolist l)) ==> not (mem_id e (diff_s (tolist b) (tolist l)))) /\
+                              (forall e. mem_id e (diff_s (tolist b) (tolist l)) ==> not (mem_id e (diff_s (tolist a) (tolist l))))) /\
+                              (sim0 (absmerge ltr atr btr) (merge ltr l atr a btr b)))
+                       (ensures (forall e e1. mem e (filter_op (fun x -> is_enqueue x && mem x ltr.l && not
+                             (exists_mem ltr.l (fun d -> is_dequeue d && mem d ltr.l && mem x ltr.l && get_id x <> get_id d && matched x d ltr))
+                               && not (exists_mem (union ltr atr).l (fun d -> is_dequeue d && mem d (union ltr atr).l && mem x (union ltr atr).l &&
+                                         get_id x <> get_id d && matched x d (union ltr atr)))
+                               && not (exists_mem (union ltr btr).l (fun d -> is_dequeue d && mem d (union ltr btr).l && mem x (union ltr btr).l &&
+                                         get_id x <> get_id d && matched x d (union ltr btr)))) ltr.l) /\
+                               mem e1 (filter_op (fun x -> is_enqueue x && mem x ltr.l && not
+                             (exists_mem ltr.l (fun d -> is_dequeue d && mem d ltr.l && mem x ltr.l && get_id x <> get_id d && matched x d ltr))
+                               && not (exists_mem (union ltr atr).l (fun d -> is_dequeue d && mem d (union ltr atr).l && mem x (union ltr atr).l &&
+                                         get_id x <> get_id d && matched x d (union ltr atr)))
+                               && not (exists_mem (union ltr btr).l (fun d -> is_dequeue d && mem d (union ltr btr).l && mem x (union ltr btr).l &&
+                                         get_id x <> get_id d && matched x d (union ltr btr)))) ltr.l) /\
+                               get_id e <> get_id e1 /\ mem e1
+                             (filter_op (fun e1 -> get_id e <> get_id e1 && ((not ((absmerge ltr atr btr).vis e e1 ||
+                               (absmerge ltr atr btr).vis e1 e) && (get_id e < get_id e1)))) (filter_op (fun x ->
+                               is_enqueue x && mem x (absmerge ltr atr btr).l && not
+                             (exists_mem (absmerge ltr atr btr).l (fun d -> is_dequeue d && mem d (absmerge ltr atr btr).l && mem x (absmerge ltr atr btr).l &&
+                               get_id x <> get_id d && matched x d (absmerge ltr atr btr)))) (absmerge ltr atr btr).l)) ==>
+                          (memq ((get_id e), (get_ele e)) (merge ltr l atr a btr b) /\ memq ((get_id e1), (get_ele e1)) (merge ltr l atr a btr b) /\
+                                get_id e <> get_id e1 /\ order ((get_id e), (get_ele e)) ((get_id e1), (get_ele e1)) (tolist (merge ltr l atr a btr b))
+                                      )))
+
+let prop_merge218 ltr l atr a btr b =
+  axiom_ae ltr; axiom_ae atr; axiom_ae btr; axiom_ae (union ltr atr); axiom_ae (union ltr btr);
+  absmerge01 ltr atr btr; prop_merge02 ltr l atr a btr b;  prop_merge01 ltr l atr a btr b; prop_merge001 ltr l atr a btr b; prop_merge002 ltr l atr a btr b;
+  prop_merge0 ltr l atr a btr b;
+  let tr = absmerge ltr atr btr in
+  let s0 = merge ltr l atr a btr b in
+  let enq_list = filter_op (fun x -> is_enqueue x && mem x tr.l && not
+                             (exists_mem tr.l (fun d -> is_dequeue d && mem d tr.l && mem x tr.l && get_id x <> get_id d && matched x d tr))) tr.l in
+
+  let enq_list6 = filter_op (fun x -> is_enqueue x && mem x ltr.l && not
+                             (exists_mem ltr.l (fun d -> is_dequeue d && mem d ltr.l && mem x ltr.l && get_id x <> get_id d && matched x d ltr))
+                               && not (exists_mem (union ltr atr).l (fun d -> is_dequeue d && mem d (union ltr atr).l && mem x (union ltr atr).l &&
+                                         get_id x <> get_id d && matched x d (union ltr atr)))
+                               && not (exists_mem (union ltr btr).l (fun d -> is_dequeue d && mem d (union ltr btr).l && mem x (union ltr btr).l &&
+                                         get_id x <> get_id d && matched x d (union ltr btr)))) ltr.l in
+
+  assert(forall e e1. mem e (enq_list6) /\ mem e1 (enq_list6) /\ get_id e <> get_id e1 /\ mem e1
+           (filter_op (fun e1 -> get_id e <> get_id e1 && ((not (tr.vis e e1 || tr.vis e1 e) && (get_id e < get_id e1)))) (enq_list)) ==>
+                          (memq ((get_id e), (get_ele e)) s0 /\ memq ((get_id e1), (get_ele e1)) s0 /\ get_id e <> get_id e1 /\
+                                      order ((get_id e), (get_ele e)) ((get_id e1), (get_ele e1)) (tolist s0)
+                                      ));
+
+  ()
+
+val prop_merge217 : ltr: ae
+                -> l:s
+                -> atr:ae
+                -> a:s
+                -> btr:ae
+                -> b:s
+                -> Lemma (requires (sorted (tolist l) /\ sorted (tolist a) /\ sorted (tolist b) /\ (forall e. mem e ltr.l ==> not (member (get_id e) atr.l)) /\
+                              (forall e. mem e ltr.l ==> not (member (get_id e) btr.l)) /\
+                              (forall e. mem e atr.l ==> not (member (get_id e) btr.l)) /\
+                              (forall e e1. (memq e a /\ memq e1 l /\ (fst e = fst e1)) ==> (snd e = snd e1)) /\
+                              (forall e e1. (memq e b /\ memq e1 l /\ (fst e = fst e1)) ==> (snd e = snd e1)) /\
+                              (forall e e1. memq e l /\ mem e1 (diff_s (tolist a) (tolist l)) ==> fst e < fst e1) /\
+                              (forall e e1. memq e l /\ mem e1 (diff_s (tolist b) (tolist l)) ==> fst e < fst e1) /\
+                            (forall e e1. mem e (tolist l) /\ mem e1 (tolist l) /\ mem e (tolist a) /\ mem e1 (tolist a) /\ order e e1 (tolist l) ==> order e e1 (tolist a)) /\
+                            (forall e e1. mem e (tolist l) /\ mem e1 (tolist l) /\ mem e (tolist b) /\ mem e1 (tolist b) /\ order e e1 (tolist l) ==> order e e1 (tolist b)) /\
+                              (forall e e1. (mem e ltr.l /\ mem e1 atr.l ==> get_id e < get_id e1)) /\
+                              (forall e e1. (mem e ltr.l /\ mem e1 btr.l ==> get_id e < get_id e1)) /\
+                              (sim ltr l /\ sim (union ltr atr) a /\ sim (union ltr btr) b) /\
+                              (forall e. mem_id e (diff_s (tolist a) (tolist l)) ==> not (mem_id e (diff_s (tolist b) (tolist l)))) /\
+                              (forall e. mem_id e (diff_s (tolist b) (tolist l)) ==> not (mem_id e (diff_s (tolist a) (tolist l))))) /\
+                              (sim0 (absmerge ltr atr btr) (merge ltr l atr a btr b)))
+                       (ensures (forall e e1. mem e (filter_op (fun x -> is_enqueue x && mem x ltr.l && not
+                             (exists_mem ltr.l (fun d -> is_dequeue d && mem d ltr.l && mem x ltr.l && get_id x <> get_id d && matched x d ltr))
+                               && not (exists_mem (union ltr atr).l (fun d -> is_dequeue d && mem d (union ltr atr).l && mem x (union ltr atr).l &&
+                                         get_id x <> get_id d && matched x d (union ltr atr)))
+                               && not (exists_mem (union ltr btr).l (fun d -> is_dequeue d && mem d (union ltr btr).l && mem x (union ltr btr).l &&
+                                         get_id x <> get_id d && matched x d (union ltr btr)))) ltr.l) /\
+                               mem e1 (filter_op (fun x -> is_enqueue x && mem x ltr.l && not
+                             (exists_mem ltr.l (fun d -> is_dequeue d && mem d ltr.l && mem x ltr.l && get_id x <> get_id d && matched x d ltr))
+                               && not (exists_mem (union ltr atr).l (fun d -> is_dequeue d && mem d (union ltr atr).l && mem x (union ltr atr).l &&
+                                         get_id x <> get_id d && matched x d (union ltr atr)))
+                               && not (exists_mem (union ltr btr).l (fun d -> is_dequeue d && mem d (union ltr btr).l && mem x (union ltr btr).l &&
+                                         get_id x <> get_id d && matched x d (union ltr btr)))) ltr.l) /\
+                               get_id e <> get_id e1 /\ mem e1
+                             (filter_op (fun e1 -> get_id e <> get_id e1 && ((absmerge ltr atr btr).vis e e1)) (filter_op (fun x ->
+                               is_enqueue x && mem x (absmerge ltr atr btr).l && not
+                             (exists_mem (absmerge ltr atr btr).l (fun d -> is_dequeue d && mem d (absmerge ltr atr btr).l && mem x (absmerge ltr atr btr).l &&
+                               get_id x <> get_id d && matched x d (absmerge ltr atr btr)))) (absmerge ltr atr btr).l)) ==>
+                          (memq ((get_id e), (get_ele e)) (merge ltr l atr a btr b) /\ memq ((get_id e1), (get_ele e1)) (merge ltr l atr a btr b) /\
+                                get_id e <> get_id e1 /\ order ((get_id e), (get_ele e)) ((get_id e1), (get_ele e1)) (tolist (merge ltr l atr a btr b))
+                                      )))
+
+let prop_merge217 ltr l atr a btr b =
+  axiom_ae ltr; axiom_ae atr; axiom_ae btr; axiom_ae (union ltr atr); axiom_ae (union ltr btr);
+  absmerge01 ltr atr btr; prop_merge02 ltr l atr a btr b;  prop_merge01 ltr l atr a btr b; prop_merge001 ltr l atr a btr b; prop_merge002 ltr l atr a btr b;
+  prop_merge0 ltr l atr a btr b;
+  let tr = absmerge ltr atr btr in
+  let s0 = merge ltr l atr a btr b in
+  let enq_list = filter_op (fun x -> is_enqueue x && mem x tr.l && not
+                             (exists_mem tr.l (fun d -> is_dequeue d && mem d tr.l && mem x tr.l && get_id x <> get_id d && matched x d tr))) tr.l in
+
+  let enq_list6 = filter_op (fun x -> is_enqueue x && mem x ltr.l && not
+                             (exists_mem ltr.l (fun d -> is_dequeue d && mem d ltr.l && mem x ltr.l && get_id x <> get_id d && matched x d ltr))
+                               && not (exists_mem (union ltr atr).l (fun d -> is_dequeue d && mem d (union ltr atr).l && mem x (union ltr atr).l &&
+                                         get_id x <> get_id d && matched x d (union ltr atr)))
+                               && not (exists_mem (union ltr btr).l (fun d -> is_dequeue d && mem d (union ltr btr).l && mem x (union ltr btr).l &&
+                                         get_id x <> get_id d && matched x d (union ltr btr)))) ltr.l in
+
+  assert(forall e e1. mem e (enq_list6) /\ mem e1 (enq_list6) /\ get_id e <> get_id e1 /\ mem e1
+           (filter_op (fun e1 -> get_id e <> get_id e1 && ((tr.vis e e1))) (enq_list)) ==>
+                          (memq ((get_id e), (get_ele e)) s0 /\ memq ((get_id e1), (get_ele e1)) s0 /\ get_id e <> get_id e1 /\
+                                      order ((get_id e), (get_ele e)) ((get_id e1), (get_ele e1)) (tolist s0)
+                                      ));
+
+  ()
 
 val prop_merge2 : ltr: ae
                 -> l:s
@@ -1352,6 +2388,66 @@ val prop_merge2 : ltr: ae
                               (forall e. mem e atr.l ==> not (member (get_id e) btr.l)) /\
                               (forall e e1. (memq e a /\ memq e1 l /\ (fst e = fst e1)) ==> (snd e = snd e1)) /\
                               (forall e e1. (memq e b /\ memq e1 l /\ (fst e = fst e1)) ==> (snd e = snd e1)) /\
+                              (forall e e1. memq e l /\ mem e1 (diff_s (tolist a) (tolist l)) ==> fst e < fst e1) /\
+                              (forall e e1. memq e l /\ mem e1 (diff_s (tolist b) (tolist l)) ==> fst e < fst e1) /\
+                            (forall e e1. mem e (tolist l) /\ mem e1 (tolist l) /\ mem e (tolist a) /\ mem e1 (tolist a) /\ order e e1 (tolist l) ==> order e e1 (tolist a)) /\
+                            (forall e e1. mem e (tolist l) /\ mem e1 (tolist l) /\ mem e (tolist b) /\ mem e1 (tolist b) /\ order e e1 (tolist l) ==> order e e1 (tolist b)) /\
+                              (forall e e1. (mem e ltr.l /\ mem e1 atr.l ==> get_id e < get_id e1)) /\
+                              (forall e e1. (mem e ltr.l /\ mem e1 btr.l ==> get_id e < get_id e1)) /\
+                              (sim ltr l /\ sim (union ltr atr) a /\ sim (union ltr btr) b) /\
+                              (forall e. mem_id e (diff_s (tolist a) (tolist l)) ==> not (mem_id e (diff_s (tolist b) (tolist l)))) /\
+                              (forall e. mem_id e (diff_s (tolist b) (tolist l)) ==> not (mem_id e (diff_s (tolist a) (tolist l))))) /\
+                              (sim0 (absmerge ltr atr btr) (merge ltr l atr a btr b)))
+                       (ensures (sim2 (absmerge ltr atr btr) (merge ltr l atr a btr b)))
+
+let prop_merge2 ltr l atr a btr b =
+  axiom_ae ltr; axiom_ae atr; axiom_ae btr; axiom_ae (union ltr atr); axiom_ae (union ltr btr);
+  absmerge01 ltr atr btr; prop_merge02 ltr l atr a btr b;  prop_merge01 ltr l atr a btr b; prop_merge001 ltr l atr a btr b;
+  prop_merge002 ltr l atr a btr b; prop_merge0 ltr l atr a btr b; prop_merge21 ltr l atr a btr b; prop_merge22 ltr l atr a btr b;
+  prop_merge23 ltr l atr a btr b; prop_merge24 ltr l atr a btr b; prop_merge25 ltr l atr a btr b; prop_merge26 ltr l atr a btr b;
+  prop_merge27 ltr l atr a btr b; prop_merge28 ltr l atr a btr b; prop_merge29 ltr l atr a btr b; prop_merge210 ltr l atr a btr b;
+  prop_merge211 ltr l atr a btr b; prop_merge212 ltr l atr a btr b; prop_merge213 ltr l atr a btr b; prop_merge214 ltr l atr a btr b;
+  prop_merge215 ltr l atr a btr b; prop_merge216 ltr l atr a btr b; prop_merge216 ltr l atr a btr b; prop_merge218 ltr l atr a btr b;
+  let tr = absmerge ltr atr btr in
+  let s0 = merge ltr l atr a btr b in
+  let enq_list = filter_op (fun x -> is_enqueue x && mem x tr.l && not
+                             (exists_mem tr.l (fun d -> is_dequeue d && mem d tr.l && mem x tr.l && get_id x <> get_id d && matched x d tr))) tr.l in
+
+  let enq_list4 = filter_op (fun x -> is_enqueue x && mem x atr.l && not
+                             (exists_mem atr.l (fun d -> is_dequeue d && mem d atr.l && mem x atr.l && get_id x <> get_id d && matched x d atr))) atr.l in
+
+  let enq_list5 = filter_op (fun x -> is_enqueue x && mem x btr.l && not
+                             (exists_mem btr.l (fun d -> is_dequeue d && mem d btr.l && mem x btr.l && get_id x <> get_id d && matched x d btr))) btr.l in
+
+  let enq_list6 = filter_op (fun x -> is_enqueue x && mem x ltr.l && not
+                             (exists_mem ltr.l (fun d -> is_dequeue d && mem d ltr.l && mem x ltr.l && get_id x <> get_id d && matched x d ltr))
+                               && not (exists_mem (union ltr atr).l (fun d -> is_dequeue d && mem d (union ltr atr).l && mem x (union ltr atr).l &&
+                                         get_id x <> get_id d && matched x d (union ltr atr)))
+                               && not (exists_mem (union ltr btr).l (fun d -> is_dequeue d && mem d (union ltr btr).l && mem x (union ltr btr).l &&
+                                         get_id x <> get_id d && matched x d (union ltr btr)))) ltr.l in
+
+  assert(forall e. mem e enq_list ==> mem e enq_list4 \/ mem e enq_list5 \/ mem e enq_list6);
+  assert(forall e e1. mem e (enq_list) /\ mem e1 (enq_list) /\ get_id e <> get_id e1 /\ mem e1
+           (filter_op (fun e1 -> get_id e <> get_id e1 && ((tr.vis e e1) || (not (tr.vis e e1 || tr.vis e1 e) && (get_id e < get_id e1)))) (enq_list)) ==>
+                          (memq ((get_id e), (get_ele e)) s0 /\ memq ((get_id e1), (get_ele e1)) s0 /\ get_id e <> get_id e1 /\
+                                      order ((get_id e), (get_ele e)) ((get_id e1), (get_ele e1)) (tolist s0)
+                                      ));
+  ()
+
+
+val prop_merge1 : ltr: ae
+                -> l:s
+                -> atr:ae
+                -> a:s
+                -> btr:ae
+                -> b:s
+                -> Lemma (requires (sorted (tolist l) /\ sorted (tolist a) /\ sorted (tolist b) /\ (forall e. mem e ltr.l ==> not (member (get_id e) atr.l)) /\
+                              (forall e. mem e ltr.l ==> not (member (get_id e) btr.l)) /\
+                              (forall e. mem e atr.l ==> not (member (get_id e) btr.l)) /\
+                              (forall e e1. (memq e a /\ memq e1 l /\ (fst e = fst e1)) ==> (snd e = snd e1)) /\
+                              (forall e e1. (memq e b /\ memq e1 l /\ (fst e = fst e1)) ==> (snd e = snd e1)) /\
+                              (forall e e1. memq e l /\ mem e1 (diff_s (tolist a) (tolist l)) ==> fst e < fst e1) /\
+                              (forall e e1. memq e l /\ mem e1 (diff_s (tolist b) (tolist l)) ==> fst e < fst e1) /\
                             (forall e e1. mem e (tolist l) /\ mem e1 (tolist l) /\ mem e (tolist a) /\ mem e1 (tolist a) /\ order e e1 (tolist l) ==> order e e1 (tolist a)) /\
                             (forall e e1. mem e (tolist l) /\ mem e1 (tolist l) /\ mem e (tolist b) /\ mem e1 (tolist b) /\ order e e1 (tolist l) ==> order e e1 (tolist b)) /\
                               (forall e e1. (mem e ltr.l /\ mem e1 atr.l ==> get_id e < get_id e1)) /\
@@ -1359,11 +2455,12 @@ val prop_merge2 : ltr: ae
                               (sim ltr l /\ sim (union ltr atr) a /\ sim (union ltr btr) b) /\
                               (forall e. mem_id e (diff_s (tolist a) (tolist l)) ==> not (mem_id e (diff_s (tolist b) (tolist l))))/\
                               (forall e. mem_id e (diff_s (tolist b) (tolist l)) ==> not (mem_id e (diff_s (tolist a) (tolist l))))))
-                       (ensures (sim2 (absmerge ltr atr btr) (merge ltr l atr a btr b)))
+                       (ensures (sim1 (absmerge ltr atr btr) (merge ltr l atr a btr b)))
 
-let prop_merge2 ltr l atr a btr b =
+
+let prop_merge1 ltr l atr a btr b =
   axiom_ae ltr; axiom_ae atr; axiom_ae btr; axiom_ae (union ltr atr); axiom_ae (union ltr btr);
-  prop_merge01 ltr l atr a btr b; prop_merge0 ltr l atr a btr b;
+  prop_merge01 ltr l atr a btr b; prop_merge001 ltr l atr a btr b; prop_merge002 ltr l atr a btr b; prop_merge0 ltr l atr a btr b;
   let tr = absmerge ltr atr btr in
   let s0 = merge ltr l atr a btr b in
   let enq_list = filter_op (fun x -> is_enqueue x && mem x tr.l && not
@@ -1380,24 +2477,39 @@ let prop_merge2 ltr l atr a btr b =
   //                            (exists_mem (union ltr btr).l (fun d -> is_dequeue d && mem d (union ltr btr).l && mem x (union ltr btr).l &&
   //                                        get_id x <> get_id d && matched x d (union ltr btr)))) (union ltr btr).l in
 
-  // let enq_list4 = filter_op (fun x -> is_enqueue x && mem x atr.l && not
-  //                            (exists_mem atr.l (fun d -> is_dequeue d && mem d atr.l && mem x atr.l && get_id x <> get_id d && matched x d atr))) atr.l in
+  let enq_list4 = filter_op (fun x -> is_enqueue x && mem x atr.l && not
+                             (exists_mem atr.l (fun d -> is_dequeue d && mem d atr.l && mem x atr.l && get_id x <> get_id d && matched x d atr))) atr.l in
 
   // let enq_list5 = filter_op (fun x -> is_enqueue x && mem x btr.l && not
   //                            (exists_mem btr.l (fun d -> is_dequeue d && mem d btr.l && mem x btr.l && get_id x <> get_id d && matched x d btr))) btr.l in
 
-  let enq_list6 = filter_op (fun x -> is_enqueue x && mem x ltr.l && not
-                             (exists_mem ltr.l (fun d -> is_dequeue d && mem d ltr.l && mem x ltr.l && get_id x <> get_id d && matched x d ltr))
-                               && not (exists_mem (union ltr atr).l (fun d -> is_dequeue d && mem d (union ltr atr).l && mem x (union ltr atr).l &&
-                                         get_id x <> get_id d && matched x d (union ltr atr)))
-                               && not (exists_mem (union ltr btr).l (fun d -> is_dequeue d && mem d (union ltr btr).l && mem x (union ltr btr).l &&
-                                         get_id x <> get_id d && matched x d (union ltr btr)))) ltr.l in
+  // let enq_list6 = filter_op (fun x -> is_enqueue x && mem x ltr.l && not
+  //                            (exists_mem ltr.l (fun d -> is_dequeue d && mem d ltr.l && mem x ltr.l && get_id x <> get_id d && matched x d ltr))
+  //                              && not (exists_mem (union ltr atr).l (fun d -> is_dequeue d && mem d (union ltr atr).l && mem x (union ltr atr).l &&
+  //                                        get_id x <> get_id d && matched x d (union ltr atr)))
+  //                              && not (exists_mem (union ltr btr).l (fun d -> is_dequeue d && mem d (union ltr btr).l && mem x (union ltr btr).l &&
+  //                                        get_id x <> get_id d && matched x d (union ltr btr)))) ltr.l in
 
-  assert(forall e. mem e (enq_list) ==> (is_enqueue e /\ (forall e1. mem e1 (filter_op (fun e1 -> is_enqueue e1 && get_id e <> get_id e1 && (tr.vis e e1)) (enq_list)) ==>
-                          (is_enqueue e1 /\ memq ((get_id e), (get_ele e)) s0 /\ memq ((get_id e1), (get_ele e1)) s0 /\ get_id e <> get_id e1 /\
-                                      order ((get_id e), (get_ele e)) ((get_id e1), (get_ele e1)) (tolist s0)
-                                      ))));
+  // assert(forall e. mem e enq_list4 ==> mem e enq_list);
 
+  assert(forall e e1. not (mem e (tolist l)) /\ mem e (tolist a) /\ not (mem e1 (tolist l)) /\ mem e1 (tolist a) /\
+           (mem e1 (filter_s (fun e1 -> fst e <> fst e1 && order e e1 (diff_s (tolist a) (tolist l)))
+                   (diff_s (tolist a) (tolist l)))) ==>
+                    (mem (fst e, Enqueue (snd e)) (enq_list) && mem (fst e1, Enqueue (snd e1)) (enq_list) && fst e <> fst e1 &&
+                       ((tr.vis (fst e, Enqueue (snd e)) (fst e1, Enqueue (snd e1))) ||
+                         (not (tr.vis (fst e, Enqueue (snd e)) (fst e1, Enqueue (snd e1)) ||
+                                tr.vis (fst e1, Enqueue (snd e1)) (fst e, Enqueue (snd e))) &&
+                   (fst e < fst e1)))));
+
+  // assert(forall e e1. mem e (tolist l) /\ mem e (tolist a) /\ mem e (tolist b) /\ mem e1 (tolist l) /\ mem e1 (tolist a) /\ mem e1 (tolist b) /\
+  //          (mem e1 (filter_s (fun e1 -> fst e <> fst e1 && order e e1 (intersection (tolist l) (tolist a) (tolist b)))
+  //                  (intersection (tolist l) (tolist a) (tolist b)))) ==>
+  //                   (mem (fst e, Enqueue (snd e)) (enq_list) && mem (fst e1, Enqueue (snd e1)) (enq_list6) && fst e <> fst e1 &&
+  //                      ((tr.vis (fst e, Enqueue (snd e)) (fst e1, Enqueue (snd e1))) ||
+  //                        (not (tr.vis (fst e, Enqueue (snd e)) (fst e1, Enqueue (snd e1)) ||
+  //                               tr.vis (fst e1, Enqueue (snd e1)) (fst e, Enqueue (snd e))) &&
+  //                  (fst e < fst e1)))
+  //          ));
   admit(); ()
 
 
@@ -1412,6 +2524,8 @@ val prop_merge : ltr: ae
                               (forall e. mem e atr.l ==> not (member (get_id e) btr.l)) /\
                               (forall e e1. (memq e a /\ memq e1 l /\ (fst e = fst e1)) ==> (snd e = snd e1)) /\
                               (forall e e1. (memq e b /\ memq e1 l /\ (fst e = fst e1)) ==> (snd e = snd e1)) /\
+                              (forall e e1. memq e l /\ mem e1 (diff_s (tolist a) (tolist l)) ==> fst e < fst e1) /\
+                              (forall e e1. memq e l /\ mem e1 (diff_s (tolist b) (tolist l)) ==> fst e < fst e1) /\
                             (forall e e1. mem e (tolist l) /\ mem e1 (tolist l) /\ mem e (tolist a) /\ mem e1 (tolist a) /\ order e e1 (tolist l) ==> order e e1 (tolist a)) /\
                             (forall e e1. mem e (tolist l) /\ mem e1 (tolist l) /\ mem e (tolist b) /\ mem e1 (tolist b) /\ order e e1 (tolist l) ==> order e e1 (tolist b)) /\
                               (forall e e1. (mem e ltr.l /\ mem e1 atr.l ==> get_id e < get_id e1)) /\
@@ -1511,6 +2625,5 @@ let prop_oper tr st op =
   prop_oper5 tr st op;
   prop_oper6 tr st op;
   ()
-
 
 
